updating PCUICEquality with a conv_pb

pcuic/theories/PCUICEquality.v
@@ -9,6 +9,62 @@ From Equations.Prop Require Import DepElim.
 From Equations Require Import Equations.
 Set Equations With UIP.
 
+(** TODO MOVE *)
+
+Inductive lt_pb : conv_pb -> conv_pb -> Type :=
+  | lt_refl pb : lt_pb pb pb
+  | lt_conv_cum : lt_pb Conv Cumul.
+
+Lemma conv_min pb : lt_pb Conv pb.
+Proof.
+  destruct pb ; now constructor.
+Qed.
+
+Lemma lt_conv pb : lt_pb pb Conv -> pb = Conv.
+Proof.
+  now inversion 1.
+Qed.
+
+Lemma gt_cumul pb : lt_pb Cumul pb -> pb = Cumul.
+Proof.
+  now inversion 1.
+Qed.
+
+#[global] Hint Resolve conv_min lt_conv gt_cumul : core.
+
+#[global] Instance lt_pb_refl : CRelationClasses.Reflexive lt_pb.
+Proof.
+  intros p.
+  now constructor.
+Qed.
+
+#[global] Instance lt_pb_trans : CRelationClasses.Transitive lt_pb.
+Proof.
+  intros p p' p''.
+  now inversion 1.
+Qed.
+
+#[global] Instance lt_pb_preord : CRelationClasses.PreOrder lt_pb.
+Proof.
+  now constructor ; tc.
+Qed.
+
+#[global] Instance lt_pb_antisym : CRelationClasses.Antisymmetric eq lt_pb.
+Proof.
+  now inversion 1.
+Qed.
+
+#[global] Instance lt_pb_partialord : CRelationClasses.PartialOrder eq lt_pb.
+Proof.
+  intros p p' ; cbn.
+  split ; intros H.
+  - now subst.
+  - destruct H as [H H'].
+    inversion H ; subst.
+    1: reflexivity.
+    inversion H'.
+Qed.
+
 Ltac pcuic :=
   try repeat red; cbn in *;
    try (solve [ intuition auto; eauto with pcuic || (try lia || congruence) ]).
@@ -19,8 +75,40 @@ Instance All2_fold_len {A} P (Γ Δ : list A) : HasLen (All2_fold P Γ Δ) #|Γ|
 
 Implicit Types (cf : checker_flags).
 
+(* TODO MOVE *)
+#[global]
+Existing Instance All2_symP.
+
+(* TODO MOVE *)
+#[global]
+Instance Forall2_symP :
+  forall A (P : A -> A -> Prop),
+    RelationClasses.Symmetric P ->
+    Symmetric (Forall2 P).
+Proof.
+  intros A P h l l' hl.
+  induction hl. all: auto.
+Qed.
+
 Definition R_universe_instance R :=
   fun u u' => Forall2 R (List.map Universe.make u) (List.map Universe.make u').
+
+#[global]
+Instance R_universe_instance_refl R : RelationClasses.Reflexive R -> 
+  RelationClasses.Reflexive (R_universe_instance R).
+Proof. intros tRe x. eapply Forall2_map. 
+  induction x; constructor; auto.
+Qed.
+
+#[global]
+Instance R_universe_instance_sym R : RelationClasses.Symmetric R -> 
+  RelationClasses.Symmetric (R_universe_instance R).
+Proof. intros tRe x y. now eapply Forall2_symP. Qed.
+
+#[global]
+Instance R_universe_instance_trans R : RelationClasses.Transitive R -> 
+  RelationClasses.Transitive (R_universe_instance R).
+Proof. intros tRe x y z. now eapply Forall2_trans. Qed.
 
 (** Cumulative inductive types:
 
@@ -29,22 +117,22 @@ Definition R_universe_instance R :=
   even on ill-formed terms. It corresponds to the right notion on well-formed terms.
 *)
 
-Definition R_universe_variance (Re Rle : Universe.t -> Universe.t -> Prop) v u u' :=
+Definition R_universe_variance (R : conv_pb -> Universe.t -> Universe.t -> Prop) pb v u u' :=
   match v with
   | Variance.Irrelevant => True
-  | Variance.Covariant => Rle (Universe.make u) (Universe.make u')
-  | Variance.Invariant => Re (Universe.make u) (Universe.make u')
+  | Variance.Covariant => R pb (Universe.make u) (Universe.make u')
+  | Variance.Invariant => R Conv (Universe.make u) (Universe.make u')
   end.
 
-Fixpoint R_universe_instance_variance Re Rle v u u' :=
+Fixpoint R_universe_instance_variance R pb v u u' :=
   match u, u' return Prop with
   | u :: us, u' :: us' =>
     match v with
-    | [] => R_universe_instance_variance Re Rle v us us' 
+    | [] => R_universe_instance_variance R pb v us us' 
       (* Missing variance stands for irrelevance, we still check that the instances have
         the same length. *)
-    | v :: vs => R_universe_variance Re Rle v u u' /\
-        R_universe_instance_variance Re Rle vs us us'
+    | v :: vs => R_universe_variance R pb v u u' /\
+        R_universe_instance_variance R pb vs us us'
     end
   | [], [] => True
   | _, _ => False
@@ -75,18 +163,18 @@ Definition global_variance Σ gr napp :=
   | _ => None
   end.
 
-Definition R_opt_variance Re Rle v :=
+Definition R_opt_variance R pb v :=
   match v with 
-  | Some v => R_universe_instance_variance Re Rle v
-  | None => R_universe_instance Re
+  | Some v => R_universe_instance_variance R pb v
+  | None => R_universe_instance (R Conv)
   end.
 
-Definition R_global_instance Σ Re Rle gr napp :=
-  R_opt_variance Re Rle (global_variance Σ gr napp).
+Definition R_global_instance Σ R pb gr napp :=
+  R_opt_variance R pb (global_variance Σ gr napp).
 
-Definition R_ind_universes {cf:checker_flags} (Σ : global_env_ext) ind n i i' :=
-  R_global_instance Σ (eq_universe (global_ext_constraints Σ))
-    (leq_universe (global_ext_constraints Σ)) (IndRef ind) n i i'.  
+Definition R_ind_universes {cf:checker_flags} (Σ : global_env_ext) pb ind n i i' :=
+  R_global_instance Σ (fun pb' => compare_universe pb' (global_ext_constraints Σ)) pb
+  (IndRef ind) n i i'.  
 
 Lemma R_universe_instance_impl R R' :
   RelationClasses.subrelation R R' ->
@@ -103,168 +191,206 @@ Proof.
 Qed.
 
 Section compare_decls.
-  (* leq_term compares types, eq_term bodies:
-    - For conversion they are both equality
-    - For cumulativity only the type are compared using leq.
-  *)
-  Context {eq_term leq_term : term -> term -> Type}.
+  (* Only the type are compared using cumulativity,
+  the bodies are always compared for conversion.
+   *)
+
+  Context {compare_term : conv_pb -> term -> term -> Type} {pb : conv_pb}.
   Inductive compare_decls  : context_decl -> context_decl -> Type :=
   | compare_vass {na T na' T'} :
     eq_binder_annot na na' ->
-    leq_term T T' ->
+    compare_term pb T T' ->
     compare_decls (vass na T) (vass na' T')
   | compare_vdef {na b T na' b' T'} :
     eq_binder_annot na na' ->
-    eq_term b b' ->
-    leq_term T T' -> 
+    compare_term Conv b b' ->
+    compare_term pb T T' -> 
     compare_decls (vdef na b T) (vdef na' b' T').
 
   Derive Signature NoConfusion for compare_decls.
 End compare_decls.
 Arguments compare_decls : clear implicits.
 
-Notation eq_context_upto_names := (All2 (compare_decls eq eq)).
+Notation eq_context_pb compare_term pb :=
+  (All2 (compare_decls compare_term pb)).
 
-Notation eq_context_gen eq_term leq_term :=
-  (All2_fold (fun _ _ => compare_decls eq_term leq_term)).
+Notation eq_context_upto_names := (eq_context_pb (fun _ => eq) Cumul).
 
-Lemma eq_context_upto_names_gen Γ Γ' : eq_context_upto_names Γ Γ' <~> eq_context_gen eq eq Γ Γ'.
+Lemma eq_context_upto_names_pb pb Γ Γ' :
+  eq_context_upto_names Γ Γ' <~> eq_context_pb (fun _ => eq) pb Γ Γ'.
 Proof.
   split; intros e; depind e; constructor; auto.
+  all: match goal with | H : compare_decls _ _ _ _ |- _ => destruct H ; now constructor end.
 Qed.
 
-Lemma compare_decls_impl eq_term leq_term eq_term' leq_term' :
-  subrelation eq_term eq_term' ->
-  subrelation leq_term leq_term' ->
-  subrelation (compare_decls eq_term leq_term)
-    (compare_decls eq_term' leq_term').
+Lemma compare_decls_impl compare_term compare_term' pb :
+  subrelation (compare_term Conv) (compare_term' Conv) ->
+  subrelation (compare_term pb) (compare_term' pb) ->
+  subrelation (compare_decls compare_term pb)
+    (compare_decls compare_term' pb).
 Proof.
   intros he hle x y []; constructor; auto.
 Qed.
 
-Lemma eq_context_gen_impl eq_term leq_term eq_term' leq_term' :
-  subrelation eq_term eq_term' ->
-  subrelation leq_term leq_term' ->
-  subrelation (eq_context_gen eq_term leq_term) (eq_context_gen eq_term' leq_term').
+Lemma eq_context_pb_impl compare_term compare_term' pb :
+subrelation (compare_term Conv) (compare_term' Conv) ->
+  subrelation (compare_term pb) (compare_term' pb) ->
+  subrelation (eq_context_pb compare_term pb) (eq_context_pb compare_term' pb).
 Proof.
-  intros he hle x y eq.
-  eapply All2_fold_impl; tea => /=.
-  intros; eapply compare_decls_impl; tea.
+  red.
+  solve_all.
+  intros; eapply compare_decls_impl ; eauto.
 Qed.
 
-Lemma compare_decl_impl_ondecl P eq_term leq_term eq_term' leq_term' d d' :
-  ondecl P d ->
-  (forall x y, P x -> eq_term x y -> eq_term' x y) ->
-  (forall x y, P x -> leq_term x y -> leq_term' x y) ->
-  compare_decls eq_term leq_term d d' ->
-  compare_decls eq_term' leq_term' d d'.
-Proof.
-  intros ond he hle cd; depelim cd; depelim ond; constructor => //; eauto.
-Qed.
-
-Lemma compare_decl_map eq_term leq_term f g d d' :
-  compare_decls (fun x y => eq_term (f x) (g y))
-    (fun x y => leq_term (f x) (g y)) d d' ->
-  compare_decls eq_term leq_term (map_decl f d) (map_decl g d').
+Lemma compare_decl_map compare_term pb f g d d' :
+  compare_decls (fun pb' x y => compare_term pb' (f x) (g y)) pb d d' ->
+  compare_decls compare_term pb (map_decl f d) (map_decl g d').
 Proof.
   intros h; depelim h; constructor; intuition auto.
 Qed.
 
-Definition bcompare_decls (eq_term leq_term : term -> term -> bool) (d d' : context_decl) : bool :=
+Definition bcompare_decls (compare_term : conv_pb -> term -> term -> bool)
+  pb (d d' : context_decl) : bool :=
   match d, d' with
   | {| decl_name := na; decl_body := None; decl_type := T |},
     {| decl_name := na'; decl_body := None; decl_type := T' |} =>
-    eqb_binder_annot na na' && leq_term T T'
+    eqb_binder_annot na na' && compare_term pb T T'
   | {| decl_name := na; decl_body := Some b; decl_type := T |},
     {| decl_name := na'; decl_body := Some b'; decl_type := T' |} =>
-    eqb_binder_annot na na' && eq_term b b' && leq_term T T'
+    eqb_binder_annot na na' && compare_term Conv b b' && compare_term pb T T'
   | _, _ => false
   end.
 
-#[global]
-Polymorphic Instance compare_decl_refl eq_term leq_term : 
-  CRelationClasses.Reflexive eq_term -> 
-  CRelationClasses.Reflexive leq_term -> 
-  CRelationClasses.Reflexive (compare_decls eq_term leq_term).    
+#[global] Polymorphic Instance compare_decl_refl compare_term pb :
+  CRelationClasses.Reflexive (compare_term Conv) ->
+  CRelationClasses.Reflexive (compare_term pb) ->
+  CRelationClasses.Reflexive (compare_decls compare_term pb).
 Proof.
-  intros heq hle d.
-  destruct d as [na [b|] ty]; constructor; auto; reflexivity.
+  intros he hle [? []] ; constructor; auto ; reflexivity.
 Qed.
 
 #[global]
-Polymorphic Instance compare_decl_sym eq_term leq_term :
-  CRelationClasses.Symmetric eq_term -> 
-  CRelationClasses.Symmetric leq_term -> 
-  CRelationClasses.Symmetric (compare_decls eq_term leq_term).    
+Polymorphic Instance compare_decl_refl_conv compare_term :
+  CRelationClasses.Reflexive (compare_term Conv) ->
+  CRelationClasses.Reflexive (compare_decls compare_term Conv).
 Proof.
-  intros heq hle d d' []; constructor; auto; now symmetry.
+  tc.
+Qed.
+
+#[global] Polymorphic Instance compare_decl_sym compare_term pb :
+  CRelationClasses.Symmetric (compare_term Conv) ->
+  CRelationClasses.Symmetric (compare_term pb) ->
+  CRelationClasses.Symmetric (compare_decls compare_term pb).
+Proof.
+  intros he hle d d' []; constructor ; symmetry ; auto.
 Qed.
 
 #[global]
-Polymorphic Instance compare_decl_trans eq_term leq_term :
-  CRelationClasses.Transitive eq_term -> 
-  CRelationClasses.Transitive leq_term -> 
-  CRelationClasses.Transitive (compare_decls eq_term leq_term).    
+Polymorphic Instance compare_decl_sym_conv compare_term :
+CRelationClasses.Symmetric (compare_term Conv) ->
+CRelationClasses.Symmetric (compare_decls compare_term Conv). 
 Proof.
-  intros hle hre x y z h h'; depelim h; depelim h'; constructor; auto;
+  tc.
+Qed.
+
+#[global]
+Polymorphic Instance compare_decl_trans compare_term pb :
+  CRelationClasses.Transitive (compare_term Conv) ->
+  CRelationClasses.Transitive (compare_term pb) ->
+  CRelationClasses.Transitive (compare_decls compare_term pb).
+Proof.
+  intros he hle x y z h h'; depelim h; depelim h'; constructor; auto;
   etransitivity; eauto.
+Qed.
+
+#[global]
+Polymorphic Instance compare_decl_trans_conv compare_term :
+  CRelationClasses.Transitive (compare_term Conv) ->
+  CRelationClasses.Transitive (compare_decls compare_term Conv).
+Proof.
+  tc.
 Qed.
 
 #[global]
 Instance alpha_eq_reflexive : CRelationClasses.Reflexive eq_context_upto_names.
 Proof.
-  intros x. eapply All2_refl. reflexivity.
+  red. intros. eapply All2_refl. reflexivity.
 Qed.
 
 #[global]
 Instance alpha_eq_symmmetric : CRelationClasses.Symmetric eq_context_upto_names.
 Proof.
-  intros x. eapply All2_symP. tc.
+  red. eapply All2_symP. tc.
 Qed.
 
 #[global]
 Instance alpha_eq_trans : CRelationClasses.Transitive eq_context_upto_names.
 Proof.
-  intros x y z. apply All2_trans. tc.
+  red. apply All2_trans. tc.
 Qed.
 
 #[global]
-Polymorphic Instance eq_context_refl eq_term leq_term : 
-  CRelationClasses.Reflexive eq_term -> 
-  CRelationClasses.Reflexive leq_term -> 
-  CRelationClasses.Reflexive (eq_context_gen eq_term leq_term).    
+Polymorphic Instance eq_context_refl compare_term pb : 
+  CRelationClasses.Reflexive (compare_term Conv) ->
+  CRelationClasses.Reflexive (compare_term pb) ->
+  CRelationClasses.Reflexive (eq_context_pb compare_term pb).    
 Proof.
-  intros heq hle x.
-  eapply All2_fold_refl.
-  intros. reflexivity. 
+  intros he hle x.
+  now eapply All2_refl.
 Qed.
 
 #[global]
-Polymorphic Instance eq_context_sym eq_term leq_term : 
-  CRelationClasses.Symmetric eq_term -> 
-  CRelationClasses.Symmetric leq_term -> 
-  CRelationClasses.Symmetric (eq_context_gen eq_term leq_term).    
+Polymorphic Instance eq_context_refl_conv compare_term : 
+  CRelationClasses.Reflexive (compare_term Conv) ->
+  CRelationClasses.Reflexive (eq_context_pb compare_term Conv).
 Proof.
-  intros heq hle x.
-  eapply All2_fold_sym.
-  intros. now symmetry. 
+  tc.
 Qed.
 
 #[global]
-Polymorphic Instance eq_context_trans eq_term leq_term : 
-  CRelationClasses.Transitive eq_term -> 
-  CRelationClasses.Transitive leq_term -> 
-  CRelationClasses.Transitive (eq_context_gen eq_term leq_term).    
+Polymorphic Instance eq_context_sym compare_term pb : 
+  CRelationClasses.Symmetric (compare_term Conv) ->
+  CRelationClasses.Symmetric (compare_term pb) ->
+  CRelationClasses.Symmetric (eq_context_pb compare_term pb).
+Proof.
+  intros ? ? ? ?.
+  eapply All2_symP ; tea.
+  red. now symmetry.
+Qed.
+
+#[global]
+Polymorphic Instance eq_context_sym_conv compare_term : 
+  CRelationClasses.Symmetric (compare_term Conv) ->
+  CRelationClasses.Symmetric (eq_context_pb compare_term Conv).
+Proof.
+  tc.
+Qed.
+
+#[global]
+Polymorphic Instance eq_context_trans compare_term pb : 
+  CRelationClasses.Transitive (compare_term Conv) ->
+  CRelationClasses.Transitive (compare_term pb) ->  
+  CRelationClasses.Transitive (eq_context_pb compare_term pb).
 Proof.
   intros hr x y z.
-  eapply All2_fold_trans; intros.
-  now transitivity y0. 
+  eapply All2_trans; intros.
+  red.
+  now etransitivity.
+Qed.
+
+
+#[global]
+Polymorphic Instance eq_context_trans_conv compare_term : 
+  CRelationClasses.Transitive (compare_term Conv) ->  
+  CRelationClasses.Transitive (eq_context_pb compare_term Conv).
+Proof.
+  tc.
 Qed.
 
 Definition eq_predicate (eq_term : term -> term -> Type) Re p p' :=
   All2 eq_term p.(pparams) p'.(pparams) *
   (R_universe_instance Re p.(puinst) p'.(puinst) *
-  ((eq_context_gen eq eq p.(pcontext) p'.(pcontext)) *
+  ((eq_context_upto_names p.(pcontext) p'.(pcontext)) *
     eq_term p.(preturn) p'.(preturn))).
 
 (** ** Syntactic ws_cumul_pb up-to universes
@@ -274,104 +400,107 @@ Definition eq_predicate (eq_term : term -> term -> Type) Re p p' :=
   that surround the current term, used to implement cumulativity of inductive types
   correctly (only fully applied constructors and inductives benefit from it). *)  
 
-Reserved Notation " Σ ⊢ t <==[ Rle , napp ] u" (at level 50, t, u at next level,
-  format "Σ  ⊢  t  <==[ Rle , napp ]  u").
+Reserved Notation " Σ ⊢ t <==[ pb , napp ] u" (at level 50, t, u at next level,
+  format "Σ  ⊢  t  <==[ pb , napp ]  u").
 
 
-Inductive eq_term_upto_univ_napp Σ (Re Rle : Universe.t -> Universe.t -> Prop) (napp : nat) : term -> term -> Type :=
+Inductive compare_term_upto_univ_napp Σ (R : conv_pb -> Universe.t -> Universe.t -> Prop)
+  (pb : conv_pb) (napp : nat) : term -> term -> Type :=
 | eq_Rel : forall n,
-    Σ ⊢ tRel n <==[ Rle , napp ] tRel n
+    Σ ⊢ tRel n <==[ pb , napp ] tRel n
 
 | eq_Evar : forall e args args',
-    All2 (eq_term_upto_univ_napp Σ Re Re 0) args args' ->
-    Σ ⊢ tEvar e args <==[ Rle , napp ] tEvar e args'
+    All2 (compare_term_upto_univ_napp Σ R Conv 0) args args' ->
+    Σ ⊢ tEvar e args <==[ pb , napp ] tEvar e args'
 
 | eq_Var : forall id,
-    Σ ⊢ tVar id <==[ Rle , napp ] tVar id
+    Σ ⊢ tVar id <==[ pb , napp ] tVar id
 
 | eq_Sort : forall s s',
-    Rle s s' ->
-    Σ ⊢ tSort s  <==[ Rle , napp ] tSort s'
+    R pb s s' ->
+    Σ ⊢ tSort s  <==[ pb , napp ] tSort s'
 
 | eq_App : forall t t' u u',
-    Σ ⊢ t <==[ Rle , S napp ] t' ->
-    Σ ⊢ u <==[ Re , 0 ] u' ->
-    Σ ⊢ tApp t u <==[ Rle , napp ] tApp t' u'
+    Σ ⊢ t <==[ pb , S napp ] t' ->
+    Σ ⊢ u <==[ Conv , 0 ] u' ->
+    Σ ⊢ tApp t u <==[ pb , napp ] tApp t' u'
 
 | eq_Const : forall c u u',
-    R_universe_instance Re u u' ->
-    Σ ⊢ tConst c u <==[ Rle , napp ] tConst c u'
+    R_universe_instance (R Conv) u u' ->
+    Σ ⊢ tConst c u <==[ pb , napp ] tConst c u'
 
 | eq_Ind : forall i u u',
-    R_global_instance Σ Re Rle (IndRef i) napp u u' ->
-    Σ ⊢ tInd i u <==[ Rle , napp ] tInd i u'
+    R_global_instance Σ R pb (IndRef i) napp u u' ->
+    Σ ⊢ tInd i u <==[ pb , napp ] tInd i u'
 
 | eq_Construct : forall i k u u',
-    R_global_instance Σ Re Rle (ConstructRef i k) napp u u' ->
-    Σ ⊢ tConstruct i k u <==[ Rle , napp ] tConstruct i k u'
+    R_global_instance Σ R pb (ConstructRef i k) napp u u' ->
+    Σ ⊢ tConstruct i k u <==[ pb , napp ] tConstruct i k u'
 
 | eq_Lambda : forall na na' ty ty' t t',
     eq_binder_annot na na' ->
-    Σ ⊢ ty <==[ Re , 0 ] ty' ->
-    Σ ⊢ t <==[ Rle , 0 ] t' ->
-    Σ ⊢ tLambda na ty t <==[ Rle , napp ] tLambda na' ty' t'
+    Σ ⊢ ty <==[ Conv , 0 ] ty' ->
+    Σ ⊢ t <==[ pb , 0 ] t' ->
+    Σ ⊢ tLambda na ty t <==[ pb , napp ] tLambda na' ty' t'
 
 | eq_Prod : forall na na' a a' b b',
     eq_binder_annot na na' ->
-    Σ ⊢ a <==[ Re , 0 ] a' ->
-    Σ ⊢ b <==[ Rle , 0 ] b' ->
-    Σ ⊢ tProd na a b <==[ Rle , napp ] tProd na' a' b'
+    Σ ⊢ a <==[ Conv , 0 ] a' ->
+    Σ ⊢ b <==[ pb , 0 ] b' ->
+    Σ ⊢ tProd na a b <==[ pb , napp ] tProd na' a' b'
 
 | eq_LetIn : forall na na' t t' ty ty' u u',
     eq_binder_annot na na' ->
-    Σ ⊢ t <==[ Re , 0 ] t' ->
-    Σ ⊢ ty <==[ Re , 0 ] ty' ->
-    Σ ⊢ u <==[ Rle , 0 ] u' ->
-    Σ ⊢ tLetIn na t ty u <==[ Rle , napp ] tLetIn na' t' ty' u'
+    Σ ⊢ t <==[ Conv , 0 ] t' ->
+    Σ ⊢ ty <==[ Conv , 0 ] ty' ->
+    Σ ⊢ u <==[ pb , 0 ] u' ->
+    Σ ⊢ tLetIn na t ty u <==[ pb , napp ] tLetIn na' t' ty' u'
 
 | eq_Case : forall indn p p' c c' brs brs',
-    eq_predicate (eq_term_upto_univ_napp Σ Re Re 0) Re p p' ->
-    Σ ⊢ c <==[ Re , 0 ] c' ->
+    eq_predicate (compare_term_upto_univ_napp Σ R Conv 0) (R Conv) p p' ->
+    Σ ⊢ c <==[ Conv , 0 ] c' ->
     All2 (fun x y =>
-      eq_context_gen eq eq (bcontext x) (bcontext y) *
-      (Σ ⊢ x.(bbody) <==[ Re , 0 ] y.(bbody))
+      eq_context_upto_names (bcontext x) (bcontext y) *
+      (Σ ⊢ x.(bbody) <==[ Conv , 0 ] y.(bbody))
     ) brs brs' ->
-    Σ ⊢ tCase indn p c brs <==[ Rle , napp ] tCase indn p' c' brs'
+    Σ ⊢ tCase indn p c brs <==[ pb , napp ] tCase indn p' c' brs'
 
 | eq_Proj : forall p c c',
-    Σ ⊢ c <==[ Re , 0 ] c' ->
-    Σ ⊢ tProj p c <==[ Rle , napp ] tProj p c'
+    Σ ⊢ c <==[ Conv , 0 ] c' ->
+    Σ ⊢ tProj p c <==[ pb , napp ] tProj p c'
 
 | eq_Fix : forall mfix mfix' idx,
     All2 (fun x y =>
-      (Σ ⊢ x.(dtype) <==[ Re , 0 ] y.(dtype)) *
-      (Σ ⊢ x.(dbody) <==[ Re , 0 ] y.(dbody)) *
+      (Σ ⊢ x.(dtype) <==[ Conv , 0 ] y.(dtype)) *
+      (Σ ⊢ x.(dbody) <==[ Conv , 0 ] y.(dbody)) *
       (x.(rarg) = y.(rarg)) *
       eq_binder_annot x.(dname) y.(dname)
     )%type mfix mfix' ->
-    Σ ⊢ tFix mfix idx <==[ Rle , napp ] tFix mfix' idx
+    Σ ⊢ tFix mfix idx <==[ pb , napp ] tFix mfix' idx
 
 | eq_CoFix : forall mfix mfix' idx,
     All2 (fun x y =>
-      (Σ ⊢ x.(dtype) <==[ Re , 0 ] y.(dtype)) *
-      (Σ ⊢ x.(dbody) <==[ Re , 0 ] y.(dbody)) *
+      (Σ ⊢ x.(dtype) <==[ Conv , 0 ] y.(dtype)) *
+      (Σ ⊢ x.(dbody) <==[ Conv , 0 ] y.(dbody)) *
       (x.(rarg) = y.(rarg)) *
       eq_binder_annot x.(dname) y.(dname)
     ) mfix mfix' ->
-    Σ ⊢ tCoFix mfix idx <==[ Rle , napp ] tCoFix mfix' idx
+    Σ ⊢ tCoFix mfix idx <==[ pb , napp ] tCoFix mfix' idx
     
-(* | eq_Prim i : eq_term_upto_univ_napp Σ Re Rle napp (tPrim i) (tPrim i) *)
-where " Σ ⊢ t <==[ Rle , napp ] u " := (eq_term_upto_univ_napp Σ _ Rle napp t u) : type_scope.
+(* | eq_Prim i : Σ ⊢ tPrim i <==[ pb , napp ] tPrim i *)
+where " Σ ⊢ t <==[ pb , napp ] u " := (compare_term_upto_univ_napp Σ _ pb napp t u) : type_scope.
 
-Notation eq_term_upto_univ Σ Re Rle := (eq_term_upto_univ_napp Σ Re Rle 0).
+Notation compare_term_upto_univ Σ R pb := (compare_term_upto_univ_napp Σ R pb 0).
+
+Derive Signature for compare_term_upto_univ_napp.
 
 (* ** Syntactic conparison up-to universes *)
 
 Definition compare_term_napp `{checker_flags} (pb : conv_pb) Σ φ napp (t u : term) :=
-  eq_term_upto_univ_napp Σ (eq_universe φ) (compare_universe pb φ) napp t u.
+  compare_term_upto_univ_napp Σ (fun pb' => compare_universe pb' φ) pb napp t u.
   
 Definition compare_term `{checker_flags} (pb : conv_pb) Σ φ (t u : term) :=
-  eq_term_upto_univ Σ (eq_universe φ) (compare_universe pb φ) t u.
+  compare_term_napp pb Σ φ 0 t u.
 
 (* ** Syntactic conversion up-to universes *)
 
@@ -389,44 +518,199 @@ Definition compare_opt_term `{checker_flags} (pb : conv_pb) Σ φ (t u : option 
   end.
 
 Definition compare_decl `{checker_flags} pb Σ φ (d d' : context_decl) :=
-  compare_decls (compare_term Conv Σ φ) (compare_term pb Σ φ) d d'.
+  compare_decls (fun pb' => compare_term pb' Σ φ) pb d d'.
 
 Notation eq_decl := (compare_decl Conv).
 Notation leq_decl := (compare_decl Cumul).
 
 Definition compare_context `{checker_flags} pb Σ φ (Γ Δ : context) :=
-  eq_context_gen (compare_term Conv Σ φ) (compare_term pb Σ φ) Γ Δ.
+  eq_context_pb (fun pb' => compare_term pb' Σ φ) pb Γ Δ.
   
 Notation eq_context := (compare_context Conv).
 Notation leq_context := (compare_context Cumul).
 
-Notation eq_context_upto Σ Re Rle := 
-  (eq_context_gen (eq_term_upto_univ Σ Re Re) (eq_term_upto_univ Σ Re Rle)).
+Notation eq_context_upto Σ R pb := 
+  (eq_context_pb (fun pb' => compare_term_upto_univ Σ R pb') pb).
 
-Lemma R_global_instance_refl Σ Re Rle gr napp u : 
-  RelationClasses.Reflexive Re ->
-  RelationClasses.Reflexive Rle ->
-  R_global_instance Σ Re Rle gr napp u u.
-Proof.
-  intros rRE rRle.
-  rewrite /R_global_instance.
-  destruct global_variance as [v|] eqn:lookup.
-  - induction u in v |- *; simpl; auto;
-    unfold R_opt_variance in IHu; destruct v; simpl; auto.
+Section Impl.
+
+  Lemma global_variance_napp_mon {Σ gr napp napp' v} : 
+    napp <= napp' ->
+    global_variance Σ gr napp = Some v ->
+    global_variance Σ gr napp' = Some v.
+  Proof.
+    intros hnapp.
+    rewrite /global_variance.
+    destruct gr; try congruence.
+    - destruct lookup_inductive as [[mdecl idec]|] => //.
+      destruct destArity as [[ctx s]|] => //.
+      elim: Nat.leb_spec => // cass indv.
+      elim: Nat.leb_spec => //. lia.
+    - destruct lookup_constructor as [[[mdecl idecl] cdecl]|] => //.
+      elim: Nat.leb_spec => // cass indv.
+      elim: Nat.leb_spec => //. lia.
+  Qed.
+
+  #[global]
+  Instance R_global_instance_impl_same_napp Σ R R' pb gr napp :
+    RelationClasses.subrelation (R Conv) (R' Conv) ->
+    RelationClasses.subrelation (R pb) (R' pb) ->
+    subrelation (R_global_instance Σ R pb gr napp) (R_global_instance Σ R' pb gr napp).
+  Proof.
+    intros he hle t t'.
+    rewrite /R_global_instance /R_opt_variance.
+    destruct global_variance as [v|] eqn:glob.
+    induction t in v, t' |- *; destruct v, t'; simpl; auto.
+    intros []; split; auto.
+    - destruct t0; simpl; auto.
+    - now eapply R_universe_instance_impl'.
+  Qed.
+
+  #[global]
+  Instance R_global_instance_impl Σ R R' pb pb' gr napp napp' :
+    RelationClasses.subrelation (R Conv) (R' Conv) ->
+    RelationClasses.subrelation (R Conv) (R' pb') ->
+    RelationClasses.subrelation (R pb) (R' pb') ->
+    napp <= napp' ->
+    subrelation (R_global_instance Σ R pb gr napp) (R_global_instance Σ R' pb' gr napp').
+  Proof.
+    intros he he' hle hnapp t t'.
+    rewrite /R_global_instance /R_opt_variance.
+    destruct global_variance as [v|] eqn:glob.
+    - rewrite (global_variance_napp_mon hnapp glob).
+      induction t in v, t' |- *; destruct v, t'; simpl; auto.
+      intros []; split; auto.
+      destruct t0; simpl; auto.
+      all: eapply h ; tea ; eauto.
+      all: reflexivity.
+    - destruct (global_variance _ _ napp') as [v|] eqn:glob'; eauto using R_universe_instance_impl'.
+      induction t in v, t' |- *; destruct v, t'; simpl; auto; intros H; inv H.
+      eauto.
+      split; auto.
+      destruct t0; simpl; auto.
+  Qed.
+
+  Lemma global_variance_empty gr napp : global_variance [] gr napp = None.
+  Proof.
+    destruct gr; auto.
+  Qed.
+
+  (** Pure syntactic equality, without cumulative inductive types subtyping *)
+
+  #[global]
+  Instance R_global_instance_empty_impl Σ R R' pb pb' gr napp napp' :
+    RelationClasses.subrelation (R Conv) (R' Conv) ->
+    RelationClasses.subrelation (R Conv) (R' pb') ->
+    RelationClasses.subrelation (R pb) (R' pb') ->
+    subrelation (R_global_instance [] R pb gr napp) (R_global_instance Σ R' pb' gr napp').
+  Proof.
+    intros he he' hle t t'.
+    rewrite /R_global_instance /R_opt_variance. simpl.
+    rewrite global_variance_empty.
+    destruct global_variance as [v|]; eauto using R_universe_instance_impl'.
+    induction t in v, t' |- *; destruct v, t'; simpl; intros H; inv H; auto.
+    simpl.
     split; auto.
-    destruct t; simpl; auto.
-  - apply Forall2_same; eauto.
-Qed.
+    destruct t0; simpl; auto.
+  Qed.
+
+  #[global]
+  Instance compare_term_upto_univ_impl Σ R R' pb pb' napp napp' :
+    RelationClasses.subrelation (R Conv) (R' Conv) ->
+    RelationClasses.subrelation (R Conv) (R' pb') ->
+    RelationClasses.subrelation (R pb) (R' pb') ->
+    napp <= napp' ->
+    subrelation (compare_term_upto_univ_napp Σ R pb napp) (compare_term_upto_univ_napp Σ R' pb' napp').
+  Proof.
+    intros he he' hle hnapp t t'.
+    induction t in pb, pb', he', hle, napp, napp', hnapp, t' |- * using term_forall_list_ind.
+    all: inversion 1; subst; constructor.
+    all: try solve [
+            eauto using R_universe_instance_impl'].
+    all: try solve [solve_all].
+    - eapply IHt1 ; tea.
+      auto with arith.
+    - eapply R_global_instance_impl. all:eauto.
+    - eapply R_global_instance_impl. all:eauto.
+    - unfold eq_predicate in *; eauto; solve_all.
+      eapply R_universe_instance_impl'; eauto.
+  Qed.
+
+  #[global]
+  Instance compare_term_upto_univ_empty_impl Σ R R' pb pb' napp napp' :
+    RelationClasses.subrelation (R Conv) (R' Conv) ->
+    RelationClasses.subrelation (R Conv) (R' pb') ->
+    RelationClasses.subrelation (R pb) (R' pb') ->
+    subrelation (compare_term_upto_univ_napp [] R pb napp) (compare_term_upto_univ_napp Σ R' pb' napp').
+  Proof.
+    intros he he' hle t t'.
+    induction t in pb, pb', he', hle, napp, napp', t' |- * using term_forall_list_ind.
+    all: inversion 1; subst; constructor.
+    all: try solve [
+            eauto using R_universe_instance_impl'].
+    all: try solve [solve_all].
+    - eapply R_global_instance_empty_impl. all:eauto.
+    - eapply R_global_instance_empty_impl. all:eauto.
+    - unfold eq_predicate in *; eauto; solve_all.
+      eapply R_universe_instance_impl'; eauto.
+  Qed.
+
+  #[global]
+  Instance compare_term_upto_univ_conv_pb Σ R pb napp napp' :
+    RelationClasses.subrelation (R Conv) (R Cumul) ->
+    napp <= napp' ->
+    subrelation (compare_term_upto_univ_napp Σ R Conv napp) (compare_term_upto_univ_napp Σ R pb napp').
+  Proof.
+    intros.
+    eapply compare_term_upto_univ_impl => //.
+    all: now destruct pb.
+  Qed.
+
+  #[global]
+  Instance eq_term_upto_univ_leq Σ R napp napp' :
+    RelationClasses.subrelation (R Conv) (R Cumul) ->
+    napp <= napp' ->
+    subrelation (compare_term_upto_univ_napp Σ R Conv napp) (compare_term_upto_univ_napp Σ R Cumul napp').
+  Proof.
+    exact _.
+  Qed.
+
+  #[global]
+  Instance eq_term_leq_term {cf:checker_flags} Σ φ
+    : subrelation (eq_term Σ φ) (leq_term Σ φ).
+  Proof.
+    eapply eq_term_upto_univ_leq ; auto; exact _.
+  Qed.
+
+  Lemma upto_eq_impl Σ R pb :
+    RelationClasses.Reflexive (R Conv) ->
+    RelationClasses.Reflexive (R pb) ->
+    subrelation (compare_term_upto_univ Σ (fun _ => eq) pb) (compare_term_upto_univ Σ R pb).
+  Proof.
+    intros he hle. eapply compare_term_upto_univ_impl ; auto.
+    all: move => ? ? -> //.
+  Qed.
+
+  Lemma compare_term_upto_univ_cst_ Σ R napp pb t t' :
+    (compare_term_upto_univ_napp Σ (fun _ => R Conv) pb napp t t') <~>
+    (compare_term_upto_univ_napp Σ R Conv napp t t').
+  Proof.
+    split ; intros.
+    all: eapply compare_term_upto_univ_impl ; [..|eassumption] ; eauto.
+    all: now red.
+  Qed.
+
+End Impl.
 
 #[global]
 Instance eq_binder_annot_equiv {A} : RelationClasses.Equivalence (@eq_binder_annot A A).
 Proof.
-  split. 
+  split.
   - red. reflexivity.
   - red; now symmetry.
   - intros x y z; unfold eq_binder_annot.
     apply transitivity.
-Qed. 
+Qed.
 
 Definition eq_binder_annot_refl {A} x : @eq_binder_annot A A x x.
 Proof. reflexivity. Qed.
@@ -434,326 +718,259 @@ Proof. reflexivity. Qed.
 #[global]
 Hint Resolve eq_binder_annot_refl : core.
 
-(* TODO MOVE *)
-#[global]
-Existing Instance All2_symP.
-
-(* TODO MOVE *)
-#[global]
-Instance Forall2_symP :
-  forall A (P : A -> A -> Prop),
-    RelationClasses.Symmetric P ->
-    Symmetric (Forall2 P).
-Proof.
-  intros A P h l l' hl.
-  induction hl. all: auto.
-Qed.
-
 Lemma eq_binder_relevances_refl (x : list aname) : All2 (on_rel eq binder_relevance) x x.
 Proof. now eapply All_All2_refl, All_refl. Qed.
 #[global]
 Hint Resolve eq_binder_relevances_refl : core.
 
-#[global]
-Instance R_universe_instance_refl Re : RelationClasses.Reflexive Re -> 
-  RelationClasses.Reflexive (R_universe_instance Re).
-Proof. intros tRe x. eapply Forall2_map. 
-  induction x; constructor; auto.
-Qed.
+Section Refl.
 
-#[global]
-Instance R_universe_instance_sym Re : RelationClasses.Symmetric Re -> 
-  RelationClasses.Symmetric (R_universe_instance Re).
-Proof. intros tRe x y. now eapply Forall2_symP. Qed.
- 
-#[global]
-Instance R_universe_instance_trans Re : RelationClasses.Transitive Re -> 
-  RelationClasses.Transitive (R_universe_instance Re).
-Proof. intros tRe x y z. now eapply Forall2_trans. Qed.
+  #[global] Instance R_global_instance_refl Σ R pb gr napp :
+    RelationClasses.Reflexive (R Conv) ->
+    RelationClasses.Reflexive (R pb) ->
+    RelationClasses.Reflexive (R_global_instance Σ R pb gr napp).
+  Proof.
+    intros he hle u.
+    rewrite /R_global_instance.
+    destruct global_variance as [v|] eqn:lookup.
+    - induction u in v |- *; simpl; auto;
+      unfold R_opt_variance in IHu; destruct v; simpl; auto.
+      split; auto.
+      destruct t; simpl; auto.
+    - apply Forall2_same; eauto.
+  Qed.
 
-Lemma onctx_eq_ctx P ctx eq_term :
-  onctx P ctx ->
-  (forall x, P x -> eq_term x x) ->
-  All2_fold (fun _ _ => compare_decls eq_term eq_term) ctx ctx.
-Proof.
-  intros onc HP.
-  induction onc.
-  - constructor; auto.
-  - constructor; auto; simpl.
-    destruct x as [na [b|] ty]; destruct p; simpl in *;
-    constructor; auto.
-Qed.
+  #[global]
+  Polymorphic Instance eq_predicate_refl Re Ru :
+    CRelationClasses.Reflexive Re ->
+    RelationClasses.Reflexive Ru ->
+    CRelationClasses.Reflexive (eq_predicate Re Ru).
+  Proof.
+    intros hre hru.
+    intros p. unfold eq_predicate; intuition auto; try reflexivity.
+    eapply All2_same; reflexivity.
+  Qed.
 
-#[global]
-Polymorphic Instance creflexive_eq A : CRelationClasses.Reflexive (@eq A).
-Proof. intro x. constructor. Qed.
-
-#[global]
-Polymorphic Instance eq_predicate_refl Re Ru :
-  CRelationClasses.Reflexive Re ->
-  RelationClasses.Reflexive Ru ->
-  CRelationClasses.Reflexive (eq_predicate Re Ru).
-Proof.
-  intros hre hru.
-  intros p. unfold eq_predicate; intuition auto; try reflexivity.
-  eapply All2_same; reflexivity.
-Qed.
-
-#[global]
-Polymorphic Instance eq_term_upto_univ_refl Σ Re Rle napp :
-  RelationClasses.Reflexive Re ->
-  RelationClasses.Reflexive Rle ->
-  Reflexive (eq_term_upto_univ_napp Σ Re Rle napp).
-Proof.
-  intros hRe hRle t.
-  induction t in napp, Rle, hRle |- * using term_forall_list_ind.
-  all: simpl.
-  all: try constructor. all: eauto.
-  all: try solve [eapply All_All2 ; eauto].
-  all: try solve [eapply Forall2_same ; eauto].
-  all: try solve [unfold eq_predicate; solve_all; eapply All_All2; eauto].
-  - apply R_global_instance_refl; auto.
-  - apply R_global_instance_refl; auto.
-  - destruct X as [? [? ?]].
+  #[global]
+  Polymorphic Instance compare_term_upto_univ_refl Σ R pb napp :
+    RelationClasses.Reflexive (R Conv) ->
+    RelationClasses.Reflexive (R pb) ->
+    Reflexive (compare_term_upto_univ_napp Σ R pb napp).
+  Proof.
+    intros he hle t.
+    induction t in hle, napp, pb |- * using term_forall_list_ind.
+    all: constructor.
+    all: try solve [eauto].
+    all: try solve [reflexivity].
+    all: try solve [eapply All_All2 ; intuition].
+    destruct X as [? [? ?]].
     unfold eq_predicate; solve_all.
-    eapply All_All2; eauto. reflexivity.
-    eapply onctx_eq_ctx in a0; eauto.
-  - eapply All_All2; eauto; simpl; intuition eauto.
-    eapply onctx_eq_ctx in a; eauto.
-  - eapply All_All2; eauto; simpl; intuition eauto.
-  - eapply All_All2; eauto; simpl; intuition eauto.
-Qed.
+    3: reflexivity.
+    2: now eapply R_universe_instance_refl.
+    eapply All_All2; eauto.
+  Qed.
 
-#[global]
-Instance compare_term_refl {cf} pb {Σ : global_env} φ : Reflexive (compare_term pb Σ φ).
-Proof. eapply eq_term_upto_univ_refl; tc. Qed.
+  #[global]
+  Polymorphic Instance compare_term_upto_univ_refl_conv Σ R napp :
+    RelationClasses.Reflexive (R Conv) ->
+    Reflexive (compare_term_upto_univ_napp Σ R Conv napp).
+  Proof.
+    tc.
+  Qed.
 
-Derive Signature for eq_term_upto_univ_napp.
+  #[global]
+  Instance compare_term_refl {cf} pb {Σ : global_env} φ : Reflexive (compare_term pb Σ φ).
+  Proof. eapply compare_term_upto_univ_refl ; tc. Qed.
 
-Lemma R_global_instance_sym Σ Re Rle gr napp u u' : 
-  RelationClasses.Symmetric Re ->
-  RelationClasses.Symmetric Rle ->
-  R_global_instance Σ Re Rle gr napp u' u ->
-  R_global_instance Σ Re Rle gr napp u u'.
-Proof.
-  intros rRE rRle.
-  rewrite /R_global_instance.
-  destruct global_variance as [v|] eqn:lookup.
-  - induction u in u', v |- *; destruct u'; simpl; auto;
-    destruct v as [|v vs]; unfold R_opt_variance in IHu; simpl; auto.
-    intros [Ra Ru']. split.
-    destruct v; simpl; auto.
-    apply IHu; auto.
-  - apply Forall2_symP; eauto.
-Qed.
- 
-Lemma onctx_eq_ctx_sym P ctx ctx' eq_term :
-  onctx P ctx ->
-  (forall x, P x -> forall y, eq_term x y -> eq_term y x) ->
-  All2_fold (fun _ _ => compare_decls eq_term eq_term) ctx ctx' ->
-  All2_fold (fun _ _ => compare_decls eq_term eq_term) ctx' ctx.
-Proof.
-  intros onc HP H1.
-  induction H1; depelim onc; constructor; intuition auto; simpl in *.
-  depelim p; depelim o; constructor; auto; try now symmetry.
-Qed.
+End Refl.
 
-#[global]
-Polymorphic Instance eq_term_upto_univ_sym Σ Re Rle napp :
-  RelationClasses.Symmetric Re ->
-  RelationClasses.Symmetric Rle ->
-  Symmetric (eq_term_upto_univ_napp Σ Re Rle napp).
-Proof.
-  intros he hle u v e.
-  pose proof (@RelationClasses.symmetry _ (@eq_binder_annot name name) _).
-  induction u in Rle, hle, v, napp, e |- * using term_forall_list_ind.
-  all: dependent destruction e.
-  all: try solve [
-    econstructor ; eauto using R_global_instance_sym ;
-    try eapply Forall2_symP ; eauto
-  ].
-  - econstructor.
-    eapply All2_All_mix_left in X as h; eauto.
-    clear a X.
-    induction h.
-    + constructor.
-    + destruct r as [h1 h2]. eapply h1 in h2 ; auto.
-  - solve_all. destruct e as (r & ? & eq & ?).
-    econstructor; rewrite ?e; unfold eq_predicate in *; solve_all; eauto.
-    eapply All2_sym; solve_all.
-    unfold R_universe_instance in r |- *.
-    eapply Forall2_symP; eauto.
-    eapply onctx_eq_ctx_sym in a1; eauto.
-    eapply All2_sym; solve_all.
-    eapply onctx_eq_ctx_sym in a0; eauto.
-  - econstructor.
-    eapply All2_All_mix_left in X as h; eauto.
-    clear a X.
-    induction h.
-    + constructor.
-    + destruct r as [[h1 h2] [[[h3 h4] h5] h6]].
-      eapply h1 in h3; auto. constructor; auto.
-  - econstructor.
-    eapply All2_All_mix_left in X as h; eauto.
-    clear a X.
-    induction h.
-    + constructor.
-    + destruct r as [[h1 h2] [[[h3 h4] h5] h6]]. eapply h1 in h3 ; auto.
-    constructor; auto.
-Qed.
+Section Sym.
 
-#[global]
-Polymorphic Instance eq_predicate_sym Re Ru :
-  CRelationClasses.Symmetric Re ->
-  RelationClasses.Symmetric Ru ->
-  CRelationClasses.Symmetric (eq_predicate Re Ru).
-Proof.
-  intros hre hru.
-  intros p. unfold eq_predicate; intuition auto; try now symmetry.
-Qed.
+  #[global]
+  Polymorphic Instance R_global_instance_sym Σ R pb gr napp : 
+    RelationClasses.Symmetric (R Conv) ->
+    RelationClasses.Symmetric (R pb) ->
+    RelationClasses.Symmetric (R_global_instance Σ R pb gr napp).
+  Proof.
+    intros re rle u u'.
+    rewrite /R_global_instance.
+    destruct global_variance as [v|] eqn:lookup.
+    - induction u in u', v |- *; destruct u'; simpl; auto;
+      destruct v as [|v vs]; unfold R_opt_variance in IHu; simpl; auto.
+      intros [Ra Ru']. split ; auto.
+      destruct v; simpl; auto.
+    - apply Forall2_symP; eauto.
+  Qed.
 
-#[global]
-Instance compare_term_sym {cf} Σ φ : Symmetric (compare_term Conv Σ φ).
-Proof.
-  now intros t u; unfold compare_term; cbn; symmetry.
-Qed.
+  #[global]
+  Polymorphic Instance compare_term_upto_univ_sym Σ pb R napp :
+    RelationClasses.Symmetric (R Conv) ->
+    RelationClasses.Symmetric (R pb) ->
+    Symmetric (compare_term_upto_univ_napp Σ R pb napp).
+  Proof.
+    intros he hle u v e.
+    pose proof (@RelationClasses.symmetry _ (@eq_binder_annot name name) _).
+    induction u in v, pb, hle, napp, e |- * using term_forall_list_ind.
+    all: dependent destruction e.
+    all: econstructor.
+    all: try solve [eauto].
+    all: try solve [now symmetry].
+    - eapply All2_All_mix_left in X as h; eauto.
+      clear a X.
+      induction h.
+      + constructor.
+      + destruct r as [h1 h2]. eapply h1 in h2 ; auto.
+    - solve_all. destruct e as (r & ? & eq & ?).
+      econstructor; rewrite ?e; unfold eq_predicate in *; solve_all; eauto.
+      + eapply All2_sym; solve_all.
+      + unfold R_universe_instance in r |- *.
+        eapply Forall2_symP; eauto.
+      + eapply All2_sym ; solve_all.
+        now symmetry.
+    - eapply All2_sym ; solve_all.
+      eapply All2_sym ; solve_all.
+      now symmetry.
+    - eapply All2_sym.
+      solve_all.
+    - eapply All2_sym.
+      solve_all.
+  Qed.
 
-#[global]
-Instance R_global_instance_trans Σ Re Rle gr napp :
-  RelationClasses.Transitive Re ->
-  RelationClasses.Transitive Rle ->
-  RelationClasses.Transitive (R_global_instance Σ Re Rle gr napp).
-Proof.
-  intros he hle x y z.
-  unfold R_global_instance, R_opt_variance.
-  destruct global_variance as [v|].
-  clear -he hle.
-  induction x in y, z, v |- *; destruct y, z, v; simpl; auto => //. eauto.
-  intros [Ra Rxy] [Rt Ryz].
-  split; eauto.
-  destruct t1; simpl in *; auto.
-  now etransitivity; eauto.
-  now etransitivity; eauto.
-  eapply Forall2_trans; auto.
-Qed.
+  #[global]
+  Instance compare_term_upto_univ_sym_conv Σ R napp :
+    RelationClasses.Symmetric (R Conv) ->
+    Symmetric (compare_term_upto_univ_napp Σ R Conv napp).
+  Proof.
+    tc.
+  Qed.
 
-Lemma onctx_eq_ctx_trans P ctx ctx' ctx'' eq_term :
-  onctx P ctx ->
-  (forall x, P x -> forall y z, eq_term x y -> eq_term y z -> eq_term x z) ->
-  All2_fold (fun _ _ => compare_decls eq_term eq_term) ctx ctx' ->
-  All2_fold (fun _ _ => compare_decls eq_term eq_term) ctx' ctx'' ->
-  All2_fold (fun _ _ => compare_decls eq_term eq_term) ctx ctx''.
-Proof.
-  intros onc HP H1; revert ctx''.
-  induction H1; depelim onc; intros ctx'' H; depelim H; constructor; intuition auto; simpl in *.
-  depelim o. depelim p0.
-  - depelim c; constructor; [now etransitivity|eauto].
-  - depelim c; constructor; [now etransitivity|eauto ..].
-Qed.
+  #[global]
+  Instance eq_term_sym {cf} Σ φ : Symmetric (eq_term Σ φ).
+  Proof.
+    intros t u e.
+    eapply compare_term_upto_univ_sym_conv; tea.
+    tc.
+  Qed.
 
-#[global]
-Polymorphic Instance eq_predicate_trans Re Ru :
-  CRelationClasses.Transitive Re ->
-  RelationClasses.Transitive Ru ->
-  CRelationClasses.Transitive (eq_predicate Re Ru).
-Proof.
-  intros hre hru.
-  intros p. unfold eq_predicate; intuition auto; try now etransitivity.
-  eapply All2_trans; tea.
-  etransitivity; tea.
-Qed.
+End Sym.
 
-#[global]
-Polymorphic Instance eq_term_upto_univ_trans Σ Re Rle napp :
-  RelationClasses.Transitive Re ->
-  RelationClasses.Transitive Rle ->
-  Transitive (eq_term_upto_univ_napp Σ Re Rle napp).
-Proof.
-  intros he hle u v w e1 e2.
-  pose proof (@RelationClasses.transitivity _ (@eq_binder_annot name name) _).
-  induction u in Rle, hle, v, w, napp, e1, e2 |- * using term_forall_list_ind.
-  all: dependent destruction e1.
-  all: try solve [ eauto ].
-  all: try solve [
-    dependent destruction e2 ; econstructor ; eauto;
-    try eapply Forall2_trans ; eauto
-  ].
-  - dependent destruction e2.
-    econstructor.
-    eapply All2_All_mix_left in X as h; eauto.
-    clear a X.
-    induction h in a0, args'0 |- *.
-    + assumption.
-    + dependent destruction a0. constructor ; eauto.
-      destruct r as [h1 h2]. eauto.
-  - dependent destruction e2.
-    constructor.
-    eapply R_global_instance_trans; eauto.
-  - dependent destruction e2.
-    constructor.
-    eapply R_global_instance_trans; eauto.
-  - dependent destruction e2.
-    unfold eq_predicate in *.
-    !!solve_all.
-    econstructor; unfold eq_predicate in *; solve_all; eauto.
-    * clear -he hh1 hh2.
-      revert hh1 hh2. generalize (pparams p), p'.(pparams), p'0.(pparams).
-      intros l l' l''.
-      induction 1 in l'' |- *; auto. intros H; depelim H. constructor; auto.
-      eapply r; eauto. apply r.
-    * etransitivity; eauto.
-    * eapply onctx_eq_ctx_trans in hh; eauto.
-      intros ???? -> ->; eauto.
-    * clear -H he a a0.
+Section Trans.
+
+  #[global]
+  Instance R_global_instance_trans Σ R pb gr napp :
+    RelationClasses.Transitive (R Conv) ->
+    RelationClasses.Transitive (R pb) ->
+    RelationClasses.Transitive (R_global_instance Σ R pb gr napp).
+  Proof.
+    intros he hle x y z.
+    unfold R_global_instance, R_opt_variance.
+    destruct global_variance as [v|].
+    - induction x in y, z, v |- *; destruct y, z, v; simpl; auto => //. 1: eauto.
+      intros [Ra Rxy] [Rt Ryz].
+      split; eauto.
+      destruct t1; simpl in *; eauto.
+    - eapply Forall2_trans; auto.
+  Qed.
+
+  #[global]
+  Polymorphic Instance compare_term_upto_univ_trans Σ R pb napp :
+    RelationClasses.Transitive (R Conv) ->
+    RelationClasses.Transitive (R pb) -> 
+    Transitive (compare_term_upto_univ_napp Σ R pb napp).
+  Proof.
+    intros he hle u v w e1 e2.
+    pose proof (@RelationClasses.transitivity _ (@eq_binder_annot name name) _).
+    induction u in hle, v, w, pb, napp, e1, e2 |- * using term_forall_list_ind.
+    all: dependent destruction e1.
+    all: try solve [ eauto ].
+    all: dependent destruction e2 ; econstructor.
+    all: try solve [ eauto ].
+    - solve_all.
+      induction a in a0, args'0 |- *.
+      + assumption.
+      + dependent destruction a0. intuition.
+    - eapply R_universe_instance_trans ; eauto. 
+    - eapply R_global_instance_trans; eauto.
+    - eapply R_global_instance_trans; eauto.
+    - unfold eq_predicate in *.
+      !!solve_all.
+      * clear -he hle hh0 hh1.
+        revert hh0 hh1. generalize (pparams p), p'.(pparams), p'0.(pparams).
+        intros l l' l''.
+        induction 1 in l'' |- *; auto. intros H; depelim H. constructor; auto.
+        eapply r; eauto. apply r.
+      * eapply R_universe_instance_trans ; eauto.
+      * etransitivity ; tea.
+        solve_all.
+    - !!solve_all.
+      clear -H he hle a a0.
       induction a in a0, brs'0 |- *.
       + assumption.
       + depelim a0. destruct p. constructor; auto.
-        destruct r as [[h1 h1'] [h2 h3]].
-        split.
-        eapply onctx_eq_ctx_trans in h1; eauto.
-        intros ???? -> ->;reflexivity.
-        eapply h1'; eauto.
-  - dependent destruction e2.
-    econstructor.
-    eapply All2_All_mix_left in X as h; eauto.
-    clear a X.
-    induction h in a0, mfix'0 |- *.
-    + assumption.
-    + dependent destruction a0. constructor ; eauto.
-      intuition eauto.
-      transitivity (rarg y); auto.
-  - dependent destruction e2.
-    econstructor.
-    eapply All2_All_mix_left in X as h; eauto.
-    clear a X.
-    induction h in a0, mfix'0 |- *.
-    + assumption.
-    + dependent destruction a0. constructor ; eauto.
-      intuition eauto.
-      transitivity (rarg y); auto.
-Qed.
+        split ; solve_all.
+        etransitivity ; tea.
+        solve_all.
+    - solve_all.
+      induction a in a0, mfix'0 |- *.
+      + assumption.
+      + dependent destruction a0. constructor ; eauto.
+        intuition eauto.
+        now etransitivity.
+    - solve_all.
+      induction a in a0, mfix'0 |- *.
+      + assumption.
+      + dependent destruction a0. constructor ; eauto.
+        intuition eauto.
+        now etransitivity.
+  Qed.
+
+  #[global]
+  Polymorphic Instance compare_term_upto_univ_trans_conv Σ R napp :
+    RelationClasses.Transitive (R Conv) ->
+    Transitive (compare_term_upto_univ_napp Σ R Conv napp).
+  Proof.
+    tc.
+  Qed.
+
+
+  #[global]
+  Instance leq_term_trans {cf} Σ φ : Transitive (leq_term Σ φ).
+  Proof. apply compare_term_upto_univ_trans; tc. Qed.
+
+  #[global]
+  Instance eq_term_trans {cf} Σ φ : Transitive (eq_term Σ φ).
+  Proof. apply compare_term_upto_univ_trans; tc. Qed.
+
+End Trans.
 
 #[global]
-Instance compare_term_trans {cf} pb Σ φ : Transitive (compare_term pb Σ φ).
-Proof. apply eq_term_upto_univ_trans; tc. Qed.
-
-#[global]
-Polymorphic Instance eq_term_upto_univ_equiv Σ Re (hRe : RelationClasses.Equivalence Re)
-  : Equivalence (eq_term_upto_univ Σ Re Re).
+Polymorphic Instance compare_term_upto_univ_equiv Σ R (hR : RelationClasses.Equivalence (R Conv))
+  : Equivalence (compare_term_upto_univ Σ R Conv).
 Proof.
-  constructor. all: exact _.
+  constructor; tc.
 Defined.
 
 #[global]
-Polymorphic Instance eq_context_equiv {cf} Σ φ : Equivalence (eq_context_gen (eq_term Σ φ) (eq_term Σ φ)).
+Polymorphic Instance eq_context_equiv {cf} Σ φ :
+  Equivalence (eq_context_pb (fun pb => compare_term pb Σ φ) Conv).
 Proof.
-  constructor; try exact _.
+  constructor; tc. 
 Qed.
 
 #[global]
-Polymorphic Instance leq_context_preord {cf} Σ φ : PreOrder (eq_context_gen (eq_term Σ φ) (leq_term Σ φ)).
+Polymorphic Instance compare_term_preord {cf} pb Σ φ :
+  PreOrder (compare_term pb Σ φ).
 Proof.
-  constructor; try exact _.
+  constructor;tc.
+  red.
+  eapply compare_term_upto_univ_trans; tc.
+Qed.  
+
+#[global]
+Polymorphic Instance leq_context_preord {cf} Σ φ pb :
+  PreOrder (eq_context_pb (fun pb => compare_term pb Σ φ) pb).
+Proof.
+  constructor; tc.
 Qed.
 
 #[global]
@@ -762,16 +979,13 @@ Proof. split; tc. Qed.
 
 #[global]
 Polymorphic Instance leq_term_preorder {cf:checker_flags} Σ φ : PreOrder (leq_term Σ φ).
-Proof. split; tc. Qed. 
+Proof. split; tc. Qed.
 
 #[global]
 Instance R_universe_instance_equiv R (hR : RelationClasses.Equivalence R)
   : RelationClasses.Equivalence (R_universe_instance R).
 Proof.
-  split.
-  - intro. apply Forall2_same. reflexivity.
-  - intros x y xy. eapply Forall2_sym, Forall2_impl; tea. now symmetry.
-  - intros x y z xy yz. eapply Forall2_trans; tea. apply hR.
+  split; tc.
 Qed.
 
 Lemma R_universe_instance_antisym Re Rle (hRe : RelationClasses.Equivalence Re) :
@@ -785,19 +999,16 @@ Proof.
 Qed.
 
 #[global]
-Instance R_global_instance_equiv Σ R (hR : RelationClasses.Equivalence R) gr napp
-  : RelationClasses.Equivalence (R_global_instance Σ R R gr napp).
+Instance R_global_instance_equiv Σ R (hR : RelationClasses.Equivalence (R Conv)) gr napp
+  : RelationClasses.Equivalence (R_global_instance Σ R Conv gr napp).
 Proof.
-  split.
-  - intro. apply R_global_instance_refl; typeclasses eauto.
-  - intros x y xy. eapply R_global_instance_sym; auto; typeclasses eauto.
-  - intros x y z xy yz. eapply R_global_instance_trans; eauto; typeclasses eauto.
+  split; tc.
 Qed.
 
 #[global]
-Instance R_global_instance_antisym Σ Re Rle (hRe : RelationClasses.Equivalence Re) gr napp :
-  RelationClasses.Antisymmetric _ Re Rle ->
-  RelationClasses.Antisymmetric _ (R_global_instance Σ Re Re gr napp) (R_global_instance Σ Re Rle gr napp).
+Instance R_global_instance_antisym Σ R pb (hRe : RelationClasses.Equivalence (R Conv)) gr napp :
+  RelationClasses.Antisymmetric _ (R Conv) (R Cumul) ->
+  RelationClasses.Antisymmetric _ (R_global_instance Σ R Conv gr napp) (R_global_instance Σ R pb gr napp).
 Proof.
   intros hR u v.
   unfold R_global_instance, R_opt_variance.
@@ -805,17 +1016,19 @@ Proof.
   induction u in l, v |- *; destruct v, l; simpl; auto.
   intros [at' uv] [ta vu]. split; auto.
   destruct t0; simpl in *; auto.
+  now destruct pb.
 Qed.  
 
-Lemma eq_term_upto_univ_antisym Σ Re Rle (hRe : RelationClasses.Equivalence Re) :
-  RelationClasses.Antisymmetric _ Re Rle ->
-  Antisymmetric (eq_term_upto_univ Σ Re Re) (eq_term_upto_univ Σ Re Rle).
+Lemma eq_term_upto_univ_antisym Σ R pb (hRe : RelationClasses.Equivalence (R Conv)) :
+  RelationClasses.Antisymmetric _ (R Conv) (R Cumul) ->
+  Antisymmetric (compare_term_upto_univ Σ R Conv) (compare_term_upto_univ Σ R pb).
 Proof.
   intros hR u v. generalize 0; intros n h h'.
   induction u in v, n, h, h' |- * using term_forall_list_ind.
   all: simpl ; inversion h ; subst; inversion h' ;
        subst ; try constructor ; auto.
-  all: eapply RelationClasses.antisymmetry; eauto.
+  2-3: eapply RelationClasses.antisymmetry; eauto.
+  now destruct pb.
 Qed.
 
 #[global]
@@ -825,22 +1038,7 @@ Proof.
   eapply eq_term_upto_univ_antisym; exact _.
 Qed.
 
-Lemma global_variance_napp_mon {Σ gr napp napp' v} : 
-  napp <= napp' ->
-  global_variance Σ gr napp = Some v ->
-  global_variance Σ gr napp' = Some v.
-Proof.
-  intros hnapp.
-  rewrite /global_variance.
-  destruct gr; try congruence.
-  - destruct lookup_inductive as [[mdecl idec]|] => //.
-    destruct destArity as [[ctx s]|] => //.
-    elim: Nat.leb_spec => // cass indv.
-    elim: Nat.leb_spec => //. lia.
-  - destruct lookup_constructor as [[[mdecl idecl] cdecl]|] => //.
-    elim: Nat.leb_spec => // cass indv.
-    elim: Nat.leb_spec => //. lia.
-Qed.
+(* TODO look at this *)
 
 #[global]
 Instance R_global_instance_impl_same_napp Σ Re Re' Rle Rle' gr napp :
@@ -994,6 +1192,8 @@ Proof.
   eapply eq_term_upto_univ_leq; auto; exact _.
 Qed.
 
+(* end look at this *)
+
 #[global]
 Instance leq_term_partial_order {cf:checker_flags} Σ φ
   : PartialOrder (eq_term Σ φ) (leq_term Σ φ).
@@ -1006,549 +1206,537 @@ Qed.
 #[global]
 Hint Constructors compare_decls : pcuic.
 
-Local Ltac lih :=
-  lazymatch goal with
-  | ih : forall Rle v n k, eq_term_upto_univ_napp _ _ _ ?u _ -> _
-    |- eq_term_upto_univ _ _ (lift _ _ ?u) _ =>
-    eapply ih
-  end.
+Section Lift.
 
-Lemma eq_term_upto_univ_lift Σ Re Rle n n' k :
-  Proper (eq_term_upto_univ_napp Σ Re Rle n' ==> eq_term_upto_univ_napp Σ Re Rle n') (lift n k).
-Proof.
-  intros u v e.
-  induction u in n', v, n, k, e, Rle |- * using term_forall_list_ind.
-  all: dependent destruction e.
-  all: try solve [cbn ; constructor ; try lih ; try assumption; solve_all].
-  - cbn. destruct e as (? & ? & e & ?).
-    constructor; unfold eq_predicate in *; simpl; !!solve_all.
-    * rewrite -?(All2_fold_length e).
-      eapply hh0; eauto.
-    * rewrite (All2_fold_length a). now eapply hh4.
-  - cbn. constructor.
-    pose proof (All2_length a).
-    solve_all. rewrite H. eauto.
-  - cbn. constructor.
-    pose proof (All2_length a).
-    solve_all. rewrite H. eauto.
-Qed.
+  Local Ltac lih :=
+    lazymatch goal with
+    | ih : forall pb v n k, compare_term_upto_univ_napp _ _ _ ?u _ -> _
+      |- compare_term_upto_univ _ _ (lift _ _ ?u) _ =>
+      eapply ih
+    end.
 
-Lemma lift_compare_term `{checker_flags} pb Σ ϕ n k t t' :
-  compare_term pb Σ ϕ t t' -> compare_term pb Σ ϕ (lift n k t) (lift n k t').
-Proof.
-  now apply eq_term_upto_univ_lift.
-Qed.
+  Lemma compare_term_upto_univ_lift Σ R pb n n' k :
+    Proper (compare_term_upto_univ_napp Σ R pb n' ==> compare_term_upto_univ_napp Σ R pb n') (lift n k).
+  Proof.
+    intros u v e.
+    induction u in n', v, n, k, e, pb |- * using term_forall_list_ind.
+    all: dependent destruction e.
+    all: try solve [cbn ; constructor ; try lih ; try assumption; solve_all].
+    - cbn. destruct e as (? & ? & e & ?).
+      constructor; unfold eq_predicate in *; simpl; !!solve_all.
+      * now rewrite -?(All2_length e).
+      * now rewrite (All2_length a).
+    - cbn. constructor.
+      pose proof (All2_length a).
+      solve_all. rewrite H. eauto.
+    - cbn. constructor.
+      pose proof (All2_length a).
+      solve_all. rewrite H. eauto.
+  Qed.
 
-Lemma lift_compare_decls `{checker_flags} pb Σ ϕ n k d d' :
-  compare_decl pb Σ ϕ d d' -> compare_decl pb Σ ϕ (lift_decl n k d) (lift_decl n k d').
-Proof.
-  intros []; constructor; cbn; intuition auto using lift_compare_term.
-Qed.
+  Lemma lift_compare_decls `{checker_flags} pb Σ ϕ n k d d' :
+    compare_decl pb Σ ϕ d d' -> compare_decl pb Σ ϕ (lift_decl n k d) (lift_decl n k d').
+  Proof.
+    intros []; constructor; cbn ; auto.
+    all: now apply compare_term_upto_univ_lift.
+  Qed.
 
-Lemma lift_compare_context `{checker_flags} pb Σ φ l l' n k :
-  compare_context pb Σ φ l l' ->
-  compare_context pb Σ φ (lift_context n k l) (lift_context n k l').
-Proof.
-  unfold compare_context.
-  induction 1; rewrite -> ?lift_context_snoc0. constructor.
-  constructor; auto. 
-  eapply lift_compare_decls in p.
-  now rewrite (All2_fold_length X).
-Qed.
+  Lemma lift_compare_context `{checker_flags} pb Σ φ l l' n k :
+    compare_context pb Σ φ l l' ->
+    compare_context pb Σ φ (lift_context n k l) (lift_context n k l').
+  Proof.
+    unfold compare_context.
+    induction 1; rewrite -> ?lift_context_snoc0. constructor.
+    constructor; auto. 
+    eapply lift_compare_decls in r.
+    now rewrite (All2_length X).
+  Qed.
 
-Lemma lift_eq_term {cf:checker_flags} Σ φ n k T U :
-  eq_term Σ φ T U -> eq_term Σ φ (lift n k T) (lift n k U).
-Proof.
-  apply eq_term_upto_univ_lift.
-Qed.
+  Lemma lift_eq_term {cf:checker_flags} Σ φ n k T U :
+    eq_term Σ φ T U -> eq_term Σ φ (lift n k T) (lift n k U).
+  Proof.
+    apply compare_term_upto_univ_lift.
+  Qed.
 
-Lemma lift_leq_term {cf:checker_flags} Σ φ n k T U :
-  leq_term Σ φ T U -> leq_term Σ φ (lift n k T) (lift n k U).
-Proof.
-  apply eq_term_upto_univ_lift.
-Qed.
+  Lemma lift_leq_term {cf:checker_flags} Σ φ n k T U :
+    leq_term Σ φ T U -> leq_term Σ φ (lift n k T) (lift n k U).
+  Proof.
+    apply compare_term_upto_univ_lift.
+  Qed.
 
-Local Ltac sih :=
-  lazymatch goal with
-  | ih : forall Rle v n x y, _ -> eq_term_upto_univ _ _ ?u _ -> _ -> _
-    |- eq_term_upto_univ _ _ (subst _ _ ?u) _ => eapply ih
-  end.
+End Lift.
 
-Lemma eq_term_upto_univ_substs Σ Re Rle napp :
-  RelationClasses.subrelation Re Rle ->
-  forall u v n l l',
-    eq_term_upto_univ_napp Σ Re Rle napp u v ->
-    All2 (eq_term_upto_univ Σ Re Re) l l' ->
-    eq_term_upto_univ_napp Σ Re Rle napp (subst l n u) (subst l' n v).
-Proof.
-  unfold RelationClasses.subrelation; intros hR u v n l l' hu hl.
-  induction u in napp, v, n, l, l', hu, hl, Rle, hR |- * using term_forall_list_ind.
-  all: dependent destruction hu.
-  all: try solve [ cbn ; constructor ; try sih ; eauto ].
-  - cbn. destruct (Nat.leb_spec0 n n0).
-    + case_eq (nth_error l (n0 - n)).
+Section Subst.
+
+  Local Ltac sih :=
+    lazymatch goal with
+    | ih : forall Rle v n x y, _ -> compare_term_upto_univ _ _ ?u _ -> _ -> _
+      |- compare_term_upto_univ _ _ (subst _ _ ?u) _ => eapply ih
+    end.
+
+  Lemma compare_term_upto_univ_substs Σ R pb napp :
+    RelationClasses.subrelation (R Conv) (R pb) ->
+    forall u v n l l',
+      compare_term_upto_univ_napp Σ R pb napp u v ->
+      All2 (compare_term_upto_univ Σ R Conv) l l' ->
+      compare_term_upto_univ_napp Σ R pb napp (subst l n u) (subst l' n v).
+  Proof.
+    unfold RelationClasses.subrelation; intros hR u v n l l' hu hl.
+    induction u in napp, v, n, l, l', hu, hl, pb, hR |- * using term_forall_list_ind.
+    all: dependent destruction hu.
+    all: try solve [ cbn ; constructor ; try sih ; eauto ].
+    - cbn. destruct (Nat.leb_spec0 n n0).
+      2: now constructor.
+      case_eq (nth_error l (n0 - n)).
       * intros t e. eapply All2_nth_error_Some in e as h ; eauto.
         destruct h as [t' [e' h]].
         rewrite e'.
-        eapply eq_term_upto_univ_lift.
-        eapply eq_term_upto_univ_leq. 3:eauto. all:auto with arith.  
+        eapply compare_term_upto_univ_lift.
+        eapply compare_term_upto_univ_impl ; [..|eassumption].
+        all: auto with arith.
+        reflexivity.
       * intros h. eapply All2_nth_error_None in h as hh ; eauto.
         rewrite hh.
         apply All2_length in hl as e. rewrite <- e.
         constructor.
-    + constructor.
-  - cbn. constructor. solve_all.
-  - cbn.
-    destruct e as (? & ? & e & ?).
-    constructor ; unfold eq_predicate; simpl; try sih ; solve_all.
-    * rewrite -(All2_fold_length e). eapply e1; eauto.
-    * rewrite (All2_fold_length a). now eapply b0.
-  - cbn. constructor ; try sih ; eauto.
-    pose proof (All2_length a).
-    solve_all. now rewrite H.
-  - cbn. constructor ; try sih ; eauto.
-    pose proof (All2_length a).
-    solve_all. now rewrite H.
-Qed.
+    - cbn. constructor. solve_all.
+    - cbn.
+      destruct e as (? & ? & e & ?).
+      constructor ; unfold eq_predicate; simpl; try sih ; solve_all.
+      * now rewrite -(All2_length e).
+      * now rewrite (All2_length a).
+    - cbn. constructor ; try sih ; eauto.
+      pose proof (All2_length a).
+      solve_all. now rewrite H.
+    - cbn. constructor ; try sih ; eauto.
+      pose proof (All2_length a).
+      solve_all. now rewrite H.
+  Qed.
 
-Lemma eq_term_upto_univ_subst Σ Re Rle :
-  RelationClasses.subrelation Re Rle ->
-  forall u v n x y,
-    eq_term_upto_univ Σ Re Rle u v ->
-    eq_term_upto_univ Σ Re Re x y ->
-    eq_term_upto_univ Σ Re Rle (u{n := x}) (v{n := y}).
-Proof.
-  intros hR u v n x y e1 e2.
-  eapply eq_term_upto_univ_substs; eauto.
-Qed.
+  Lemma compare_term_upto_univ_subst Σ R pb :
+    RelationClasses.subrelation (R Conv) (R pb) ->
+    forall u v n x y,
+      compare_term_upto_univ Σ R pb u v ->
+      compare_term_upto_univ Σ R Conv x y ->
+      compare_term_upto_univ Σ R pb (u{n := x}) (v{n := y}).
+  Proof.
+    intros hR u v n x y e1 e2.
+    eapply compare_term_upto_univ_substs; eauto.
+  Qed.
 
-Lemma subst_eq_term {cf:checker_flags} Σ φ l k T U :
-  eq_term Σ φ T U ->
-  eq_term Σ φ (subst l k T) (subst l k U).
-Proof.
-  intros Hleq.
-  eapply eq_term_upto_univ_substs; try easy.
-  now eapply All2_same.
-Qed.
+  Lemma subst_compare_term {cf:checker_flags} pb Σ φ l k T U :
+    compare_term pb Σ φ T U ->
+    compare_term pb Σ φ (subst l k T) (subst l k U).
+  Proof.
+    intros Hleq.
+    eapply compare_term_upto_univ_substs; try easy.
+    1: cbn ; tc.
+    now eapply All2_same.
+  Qed.
 
-Lemma subst_leq_term {cf:checker_flags} Σ φ l k T U :
-  leq_term Σ φ T U ->
-  leq_term Σ φ (subst l k T) (subst l k U).
-Proof.
-  intros Hleq.
-  eapply eq_term_upto_univ_substs; try easy.
-  intro; apply eq_universe_leq_universe.
-  now eapply All2_same.
-Qed.
+End Subst.
 
 (** ** Behavior on mkApps and it_mkLambda_or_LetIn **  *)
 
-Lemma eq_term_eq_term_napp Σ Re Rle napp t t' :
-  RelationClasses.subrelation Re Rle ->
-  eq_term_upto_univ Σ Re Rle t t' -> 
-  eq_term_upto_univ_napp Σ Re Rle napp t t'.
-Proof.
-  intros. eapply eq_term_upto_univ_impl. 5:eauto.
-  4:auto with arith. all:typeclasses eauto.
-Qed.
+Section Mk.
 
-Lemma leq_term_leq_term_napp Σ Re Rle napp t t' :
-  RelationClasses.subrelation Re Rle ->
-  eq_term_upto_univ Σ Re Rle t t' -> 
-  eq_term_upto_univ_napp Σ Re Rle napp t t'.
-Proof.
-  intros. eapply eq_term_upto_univ_impl. 5:eauto.
-  4:auto with arith. all:try typeclasses eauto.
-Qed.
+  Lemma compare_term_compare_term_napp Σ R pb napp t t' :
+    RelationClasses.subrelation (R Conv) (R pb) ->
+    compare_term_upto_univ Σ R pb t t' -> 
+    compare_term_upto_univ_napp Σ R pb napp t t'.
+  Proof.
+    intros. eapply compare_term_upto_univ_impl ; [..|eassumption].
+    all: auto with arith.
+    all: reflexivity.
+  Qed.
 
-Lemma eq_term_upto_univ_napp_mkApps Σ Re Rle u1 l1 u2 l2 napp :
-    eq_term_upto_univ_napp Σ Re Rle (#|l1| + napp) u1 u2 ->
-    All2 (eq_term_upto_univ Σ Re Re) l1 l2 ->
-    eq_term_upto_univ_napp Σ Re Rle napp (mkApps u1 l1) (mkApps u2 l2).
-Proof.
-  intros hu hl. induction l1 in napp, u1, u2, l2, hu, hl |- *.
-  - inversion hl. subst. assumption.
-  - inversion hl. subst. simpl.
-    eapply IHl1.
-    + constructor. all: assumption.
-    + assumption.
-Qed.
+  Lemma compare_term_upto_univ_napp_mkApps Σ R pb u1 l1 u2 l2 napp :
+      compare_term_upto_univ_napp Σ R pb (#|l1| + napp) u1 u2 ->
+      All2 (compare_term_upto_univ Σ R Conv) l1 l2 ->
+      compare_term_upto_univ_napp Σ R pb napp (mkApps u1 l1) (mkApps u2 l2).
+  Proof.
+    intros hu hl. induction l1 in napp, u1, u2, l2, hu, hl |- *.
+    - inversion hl. subst. assumption.
+    - inversion hl. subst. simpl.
+      eapply IHl1.
+      + constructor. all: assumption.
+      + assumption.
+  Qed.
 
-Lemma eq_term_upto_univ_napp_mkApps_l_inv Σ Re Rle napp u l t :
-    eq_term_upto_univ_napp Σ Re Rle napp (mkApps u l) t ->
-    ∑ u' l',
-      eq_term_upto_univ_napp Σ Re Rle (#|l| + napp) u u' *
-      All2 (eq_term_upto_univ Σ Re Re) l l' *
-      (t = mkApps u' l').
-Proof.
-  intros h. induction l in napp, u, t, h, Rle |- *.
-  - cbn in h. exists t, []. split ; auto.
-  - cbn in h. apply IHl in h as [u' [l' [[h1 h2] h3]]].
-    dependent destruction h1. subst.
-    eexists. eexists. split; [ split | ].
-    + eassumption.
-    + constructor.
-      * eassumption.
-      * eassumption.
-    + cbn. reflexivity.
-Qed.
+  Lemma compare_term_upto_univ_napp_mkApps_l_inv Σ R pb napp u l t :
+      compare_term_upto_univ_napp Σ R pb napp (mkApps u l) t ->
+      ∑ u' l',
+        compare_term_upto_univ_napp Σ R pb (#|l| + napp) u u' *
+        All2 (compare_term_upto_univ Σ R Conv) l l' *
+        (t = mkApps u' l').
+  Proof.
+    intros h. induction l in napp, u, t, h, pb |- *.
+    - cbn in h. exists t, []. split ; auto.
+    - cbn in h. apply IHl in h as [u' [l' [[h1 h2] h3]]].
+      dependent destruction h1. subst.
+      eexists. eexists. split; [ split | ].
+      + eassumption.
+      + constructor.
+        * eassumption.
+        * eassumption.
+      + cbn. reflexivity.
+    Qed.
 
-Lemma eq_term_upto_univ_napp_mkApps_r_inv Σ Re Rle napp u l t :
-    eq_term_upto_univ_napp Σ Re Rle napp t (mkApps u l) ->
-    ∑ u' l',
-      eq_term_upto_univ_napp Σ Re Rle (#|l| + napp) u' u *
-      All2 (eq_term_upto_univ Σ Re Re) l' l *
-      (t = mkApps u' l').
-Proof.
-  intros h. induction l in napp, u, t, h, Rle |- *.
-  - cbn in h. exists t, []. split ; auto.
-  - cbn in h. apply IHl in h as [u' [l' [[h1 h2] h3]]].
-    dependent destruction h1. subst.
-    eexists. eexists. split; [ split | ].
-    + eassumption.
-    + constructor.
-      * eassumption.
-      * eassumption.
-    + cbn. reflexivity.
-Qed.
+  Lemma compare_term_upto_univ_napp_mkApps_r_inv Σ R pb napp u l t :
+      compare_term_upto_univ_napp Σ R pb napp t (mkApps u l) ->
+      ∑ u' l',
+        compare_term_upto_univ_napp Σ R pb (#|l| + napp) u' u *
+        All2 (compare_term_upto_univ Σ R Conv) l' l *
+        (t = mkApps u' l').
+  Proof.
+    intros h. induction l in napp, u, t, h, R, pb |- *.
+    - cbn in h. exists t, []. split ; auto.
+    - cbn in h. apply IHl in h as [u' [l' [[h1 h2] h3]]].
+      dependent destruction h1. subst.
+      eexists. eexists. split; [ split | ].
+      + eassumption.
+      + constructor.
+        * eassumption.
+        * eassumption.
+      + cbn. reflexivity.
+  Qed.
 
-Lemma eq_term_upto_univ_mkApps Σ Re Rle u1 l1 u2 l2 :
-    eq_term_upto_univ_napp Σ Re Rle #|l1| u1 u2 ->
-    All2 (eq_term_upto_univ Σ Re Re) l1 l2 ->
-    eq_term_upto_univ Σ Re Rle (mkApps u1 l1) (mkApps u2 l2).
-Proof.
-  intros; apply eq_term_upto_univ_napp_mkApps; rewrite ?Nat.add_0_r; auto.
-Qed.
+  Lemma compare_term_upto_univ_mkApps Σ R pb u1 l1 u2 l2 :
+      compare_term_upto_univ_napp Σ R pb #|l1| u1 u2 ->
+      All2 (compare_term_upto_univ Σ R Conv) l1 l2 ->
+      compare_term_upto_univ Σ R pb (mkApps u1 l1) (mkApps u2 l2).
+  Proof.
+    intros; apply compare_term_upto_univ_napp_mkApps; rewrite ?Nat.add_0_r; auto.
+  Qed.
 
-Lemma eq_term_upto_univ_mkApps_l_inv Σ Re Rle u l t :
-    eq_term_upto_univ Σ Re Rle (mkApps u l) t ->
-    ∑ u' l',
-      eq_term_upto_univ_napp Σ Re Rle #|l| u u' *
-      All2 (eq_term_upto_univ Σ Re Re) l l' *
-      (t = mkApps u' l').
-Proof.
-  intros H; apply eq_term_upto_univ_napp_mkApps_l_inv in H; rewrite ?Nat.add_0_r in H; auto.
-Qed.
+  Lemma compare_term_upto_univ_mkApps_l_inv Σ R pb u l t :
+      compare_term_upto_univ Σ R pb (mkApps u l) t ->
+      ∑ u' l',
+        compare_term_upto_univ_napp Σ R pb #|l| u u' *
+        All2 (compare_term_upto_univ Σ R Conv) l l' *
+        (t = mkApps u' l').
+  Proof.
+    intros H; apply compare_term_upto_univ_napp_mkApps_l_inv in H; rewrite ?Nat.add_0_r in H; auto.
+  Qed.
 
-Lemma eq_term_upto_univ_mkApps_r_inv Σ Re Rle u l t :
-    eq_term_upto_univ Σ Re Rle t (mkApps u l) ->
-    ∑ u' l',
-      eq_term_upto_univ_napp Σ Re Rle #|l| u' u *
-      All2 (eq_term_upto_univ Σ Re Re) l' l *
-      (t = mkApps u' l').
-Proof.
-  intros H; apply eq_term_upto_univ_napp_mkApps_r_inv in H;
-    rewrite Nat.add_0_r in H; auto.
-Qed.
+  Lemma compare_term_upto_univ_mkApps_r_inv Σ R pb u l t :
+      compare_term_upto_univ Σ R pb t (mkApps u l) ->
+      ∑ u' l',
+        compare_term_upto_univ_napp Σ R pb #|l| u' u *
+        All2 (compare_term_upto_univ Σ R Conv) l' l *
+        (t = mkApps u' l').
+  Proof.
+    intros H; apply compare_term_upto_univ_napp_mkApps_r_inv in H;
+      rewrite Nat.add_0_r in H; auto.
+  Qed.
 
-Lemma R_universe_instance_eq {u u'} : R_universe_instance eq u u' -> u = u'.
-Proof.
-  intros H.
-  apply Forall2_eq in H. apply map_inj in H ; revgoals.
-  { apply Universe.make_inj. }
-  subst. constructor ; auto.
-Qed.
+  Lemma compare_term_upto_univ_isApp Σ R pb napp u v :
+    compare_term_upto_univ_napp Σ R pb napp u v ->
+    isApp u = isApp v.
+  Proof.
+    induction 1.
+    all: reflexivity.
+  Qed.
 
-Lemma valid_constraints_empty {cf} i : 
-  valid_constraints (empty_ext empty_global_env) (subst_instance_cstrs i (empty_ext empty_global_env)).
-Proof.
-  red. destruct check_univs => //.
-Qed.
+  Lemma compare_term_upto_univ_mkApps_inv Σ R pb u l u' l' :
+    isApp u = false ->
+    isApp u' = false ->
+    compare_term_upto_univ Σ R pb (mkApps u l) (mkApps u' l') ->
+    compare_term_upto_univ_napp Σ R pb #|l| u u' * All2 (compare_term_upto_univ Σ R Conv) l l'.
+  Proof.
+    intros hu hu' h.
+    apply compare_term_upto_univ_mkApps_l_inv in h as hh.
+    destruct hh as [v [args [[h1 h2] h3]]].
+    apply compare_term_upto_univ_isApp in h1 as hh1. rewrite hu in hh1.
+    apply mkApps_notApp_inj in h3 ; auto.
+    destruct h3 as [? ?]. subst. split ; auto.
+  Qed.
 
-Lemma upto_eq_impl Σ Re Rle :
-  RelationClasses.Reflexive Re ->
-  RelationClasses.Reflexive Rle ->
-  subrelation (eq_term_upto_univ Σ eq eq) (eq_term_upto_univ Σ Re Rle).
-Proof.
-  intros he hle. eapply eq_term_upto_univ_impl. 4:auto.
-  all: intros ? ? []; eauto.
-Qed.
+  Lemma compare_term_upto_univ_it_mkLambda_or_LetIn Σ R pb :
+    RelationClasses.Reflexive (R Conv) ->
+    Proper (eq_context_upto Σ R Conv ==> compare_term_upto_univ Σ R pb ==> compare_term_upto_univ Σ R pb) it_mkLambda_or_LetIn.
+  Proof.
+    intros he Γ Δ eq u v h.
+    induction eq in u, v, h, he |- *.
+    - assumption.
+    - simpl. cbn. apply IHeq => //.
+      destruct r; cbn; constructor ; tas; try reflexivity.
+  Qed.
+
+  Lemma compare_term_upto_univ_it_mkLambda_or_LetIn_r Σ R pb Γ :
+    RelationClasses.Reflexive (R Conv) ->
+    respectful (compare_term_upto_univ Σ R pb) (compare_term_upto_univ Σ R pb)
+              (it_mkLambda_or_LetIn Γ) (it_mkLambda_or_LetIn Γ).
+  Proof.
+    intros he u v h.
+    induction Γ as [| [na [b|] A] Γ ih ] in u, v, h |- *.
+    - assumption.
+    - simpl. cbn. apply ih. constructor ; try reflexivity.
+      all: auto.
+    - simpl. cbn. apply ih. constructor ; try reflexivity.
+      all: auto.
+  Qed.
+
+  Lemma compare_term_it_mkLambda_or_LetIn {cf:checker_flags} Σ pb φ Γ :
+    respectful (compare_term pb Σ φ) (compare_term pb Σ φ)
+              (it_mkLambda_or_LetIn Γ) (it_mkLambda_or_LetIn Γ).
+  Proof.
+    apply compare_term_upto_univ_it_mkLambda_or_LetIn_r; exact _.
+  Qed.
+
+  Lemma compare_term_upto_univ_it_mkProd_or_LetIn Σ R pb Γ :
+    RelationClasses.Reflexive (R Conv) ->
+    respectful (compare_term_upto_univ Σ R pb) (compare_term_upto_univ Σ R pb)
+              (it_mkProd_or_LetIn Γ) (it_mkProd_or_LetIn Γ).
+  Proof.
+    intros he u v h.
+    induction Γ as [| [na [b|] A] Γ ih ] in u, v, h |- *.
+    - assumption.
+    - simpl. cbn. apply ih. constructor ; try reflexivity.
+      all: auto.
+    - simpl. cbn. apply ih. constructor ; try reflexivity.
+      all: auto.
+  Qed.
+
+  Lemma compare_term_it_mkProd_or_LetIn {cf:checker_flags} Σ pb φ Γ:
+    respectful (compare_term pb Σ φ) (compare_term pb Σ φ)
+              (it_mkProd_or_LetIn Γ) (it_mkProd_or_LetIn Γ).
+  Proof.
+    eapply compare_term_upto_univ_it_mkProd_or_LetIn ; exact _.
+  Qed.
+
+  Lemma compare_term_it_mkLambda_or_LetIn_inv {cf:checker_flags} Σ pb φ Γ u v :
+      compare_term Σ pb φ (it_mkLambda_or_LetIn Γ u) (it_mkLambda_or_LetIn Γ v) ->
+      compare_term Σ pb φ u v.
+  Proof.
+    revert u v. induction Γ as [| [na [b|] A] Γ ih ] ; intros u v h.
+    - assumption.
+    - simpl in h. cbn in h. apply ih in h. inversion h. subst.
+      assumption.
+    - simpl in h. cbn in h. apply ih in h. inversion h. subst.
+      assumption.
+  Qed.
+
+End Mk.
 
 (** ** Syntactic ws_cumul_pb up to printing anotations ** *)
 
-Definition upto_names := eq_term_upto_univ empty_global_env eq eq.
 
-Infix "≡" := upto_names (at level 70).
+Definition upto_names := compare_term_upto_univ [] (fun _ => eq) Conv.
 
-Infix "≡'" := (eq_term_upto_univ empty_global_env eq eq) (at level 70).
-Notation upto_names' := (eq_term_upto_univ empty_global_env eq eq).
+Notation "`≡α`" := upto_names.
+Infix "≡α" := upto_names (at level 60).
+Notation "`≡Γ`" := (eq_context_upto [] (fun _ => eq) Conv).
+Infix "≡Γ" := (eq_context_upto [] (fun _ => eq) Conv) (at level 20, no associativity).
 
-#[global]
-Instance upto_names_ref : Reflexive upto_names.
-Proof.
-  eapply eq_term_upto_univ_refl; exact _.
-Qed.
+Section UptoNames.
 
-#[global]
-Instance upto_names_sym : Symmetric upto_names.
-Proof.
-  eapply eq_term_upto_univ_sym; exact _.
-Qed.
+  Lemma R_universe_instance_eq {u u'} : R_universe_instance eq u u' -> u = u'.
+  Proof.
+    intros H.
+    apply Forall2_eq in H. apply map_inj in H ; revgoals.
+    { apply Universe.make_inj. }
+    subst. constructor ; auto.
+  Qed.
 
-#[global]
-Instance upto_names_trans : Transitive upto_names.
-Proof.
-  eapply eq_term_upto_univ_trans; exact _.
-Qed.
+  Lemma valid_constraints_empty {cf} i : valid_constraints (empty_ext []) (subst_instance_cstrs i (empty_ext [])).
+  Proof.
+    red. destruct check_univs => //.
+  Qed.
 
-(* todo: rename *)
-(* Definition nleq_term t t' := *)
-(*   eqb_term_upto_univ eqb eqb t t'. *)
+  #[global]
+  Instance upto_names_terms_refl : CRelationClasses.Reflexive (All2 `≡α`).
+  Proof. intro; apply All2_refl; reflexivity. Qed.
 
-(* Corollary reflect_upto_names : *)
-(*   forall t t', reflectT (upto_names t t') (nleq_term t t'). *)
-(* Proof. *)
-(*   intros t t'. eapply reflect_eq_term_upto_univ. *)
-(*   all: intros u u'; eapply reflect_reflectT, eqb_spec. *)
-(* Qed. *)
+  Lemma eq_context_upto_empty_impl {cf} {Σ : global_env_ext} pb ctx ctx' :
+    ctx ≡Γ ctx' ->
+    eq_context_upto Σ (fun _ => eq_universe Σ) pb ctx ctx'.
+  Proof.
+    intros. solve_all.
+    destruct X ; constructor ; auto.
+    all: eapply compare_term_upto_univ_empty_impl; eauto. 
+    all: move => ? ? -> ; reflexivity.
+  Qed.
 
-Lemma upto_names_impl Σ Re Rle :
-  RelationClasses.Reflexive Re ->
-  RelationClasses.Reflexive Rle ->
-  subrelation upto_names (eq_term_upto_univ Σ Re Rle).
-Proof.
-  intros he hle. eapply eq_term_upto_univ_empty_impl; auto.
-  all: intros ? ? []; eauto.
-Qed.
+  (* Infix "≡'" := (eq_term_upto_univ [] eq eq) (at level 70).
+  Notation upto_names' := (eq_term_upto_univ [] eq eq). *)
 
-Lemma upto_names_impl_eq_term {cf:checker_flags} Σ φ u v :
-    u ≡ v -> eq_term Σ φ u v.
-Proof.
-  eapply upto_names_impl ; exact _.
-Qed.
+  #[global]
+  Instance upto_names_ref : Reflexive upto_names.
+  Proof.
+    tc.
+  Qed.
 
-Lemma upto_names_impl_leq_term {cf:checker_flags} Σ φ u v :
-    u ≡ v -> leq_term Σ φ u v.
-Proof.
-  eapply upto_names_impl ; exact _.
-Qed.
+  #[global]
+  Instance upto_names_sym : Symmetric upto_names.
+  Proof.
+    tc.
+  Qed.
 
-Lemma eq_term_upto_univ_isApp Σ Re Rle napp u v :
-  eq_term_upto_univ_napp Σ Re Rle napp u v ->
-  isApp u = isApp v.
-Proof.
-  induction 1.
-  all: reflexivity.
-Qed.
+  #[global]
+  Instance upto_names_trans : Transitive upto_names.
+  Proof.
+    tc.
+  Qed.
 
-(** ** ws_cumul_pb on contexts ** *)
+  Lemma upto_names_impl Σ R pb :
+    RelationClasses.Reflexive (R Conv) ->
+    RelationClasses.Reflexive (R pb) ->
+    subrelation upto_names (compare_term_upto_univ Σ R pb).
+  Proof.
+    intros h h'.
+    eapply compare_term_upto_univ_empty_impl; auto.
+    all: red in h, h' |- * => ? ? -> //.
+  Qed.
 
-Inductive rel_option {A B} (R : A -> B -> Type) : option A -> option B -> Type :=
-| rel_some : forall a b, R a b -> rel_option R (Some a) (Some b)
-| rel_none : rel_option R None None.
+  Lemma upto_names_impl_eq_term {cf:checker_flags} Σ φ u v :
+      u ≡α v -> eq_term Σ φ u v.
+  Proof.
+    eapply upto_names_impl ; exact _.
+  Qed.
 
-Derive Signature NoConfusion for rel_option.
+  Lemma upto_names_impl_leq_term {cf:checker_flags} Σ φ u v :
+      u ≡α v -> leq_term Σ φ u v.
+  Proof.
+    eapply upto_names_impl ; exact _.
+  Qed.
 
-Definition eq_decl_upto_gen Σ Re Rle d d' : Type :=
-  eq_binder_annot d.(decl_name) d'.(decl_name) *
-  rel_option (eq_term_upto_univ Σ Re Re) d.(decl_body) d'.(decl_body) *
-  eq_term_upto_univ Σ Re Rle d.(decl_type) d'.(decl_type).
+End UptoNames.
 
-(* TODO perhaps should be def *)
-Lemma All2_eq_context_upto Σ Re Rle :
-  subrelation (All2 (eq_decl_upto_gen Σ Re Rle)) (eq_context_upto Σ Re Rle).
-Proof.
-  intros Γ Δ h.
-  induction h.
-  - constructor.
-  - destruct r as [[h1 h2] h3].
-    destruct x as [na bo ty], y as [na' bo' ty'].
-    simpl in h1, h2.
-    destruct h2.
-    + constructor ; eauto. constructor; auto.
-    + constructor ; eauto. constructor; auto.
-Qed.
+  (** ** ws_cumul_pb on contexts ** *)
 
-Lemma eq_context_upto_refl Σ Re Rle :
-  RelationClasses.Reflexive Re ->
-  RelationClasses.Reflexive Rle ->
-  Reflexive (eq_context_upto Σ Re Rle).
-Proof. exact _. Qed.
+  (* Inductive rel_option {A B} (R : A -> B -> Type) : option A -> option B -> Type :=
+  | rel_some : forall a b, R a b -> rel_option R (Some a) (Some b)
+  | rel_none : rel_option R None None.
 
-Lemma eq_context_upto_sym Σ Re Rle :
-  RelationClasses.Symmetric Re ->
-  RelationClasses.Symmetric Rle ->
-  Symmetric (eq_context_upto Σ Re Rle).
-Proof. exact _. Qed.
+  Derive Signature NoConfusion for rel_option.
 
-Lemma eq_context_upto_cat Σ Re Rle Γ Δ Γ' Δ' :
-  eq_context_upto Σ Re Rle Γ Γ' ->
-  eq_context_upto Σ Re Rle Δ Δ' ->
-  eq_context_upto Σ Re Rle (Γ ,,, Δ) (Γ' ,,, Δ').
-Proof. intros. eapply All2_fold_app; eauto. Qed.
+  Definition eq_decl_upto_gen Σ R pb d d' : Type :=
+    eq_binder_annot d.(decl_name) d'.(decl_name) *
+    rel_option (eq_term_upto_univ Σ Re Re) d.(decl_body) d'.(decl_body) *
+    eq_term_upto_univ Σ Re Rle d.(decl_type) d'.(decl_type).
 
-Lemma eq_context_upto_rev Σ Re Rle Γ Δ :
-  eq_context_upto Σ Re Rle Γ Δ ->
-  eq_context_upto Σ Re Rle (rev Γ) (rev Δ).
-Proof.
-  induction 1.
-  - constructor.
-  - rewrite 2!rev_cons. eapply eq_context_upto_cat ; eauto.
-    constructor ; eauto. constructor.
-Qed.
+  (* TODO perhaps should be def *)
+  Lemma All2_eq_context_upto Σ Re Rle :
+    subrelation (All2 (eq_decl_upto_gen Σ Re Rle)) (eq_context_upto Σ Re Rle).
+  Proof.
+    intros Γ Δ h.
+    induction h.
+    - constructor.
+    - destruct r as [[h1 h2] h3].
+      destruct x as [na bo ty], y as [na' bo' ty'].
+      simpl in h1, h2.
+      destruct h2.
+      + constructor ; eauto. constructor; auto.
+      + constructor ; eauto. constructor; auto.
+  Qed. *)
 
-Lemma eq_context_upto_rev' :
-  forall Σ Γ Δ Re Rle,
-    eq_context_upto Σ Re Rle Γ Δ ->
-    eq_context_upto Σ Re Rle (List.rev Γ) (List.rev Δ).
-Proof.
-  intros Σ Γ Δ Re Rle h.
-  induction h.
-  - constructor.
-  - simpl. eapply eq_context_upto_cat.
-    + repeat constructor; assumption.
-    + assumption.
-Qed.
+  Lemma eq_context_upto_refl Σ R pb :
+    RelationClasses.Reflexive (R Conv) ->
+    RelationClasses.Reflexive (R pb) ->
+    Reflexive (eq_context_upto Σ R pb).
+  Proof.
+    tc.
+  Qed.
 
-Lemma eq_context_upto_length :
-  forall {Σ Re Rle Γ Δ},
-    eq_context_upto Σ Re Rle Γ Δ ->
-    #|Γ| = #|Δ|.
-Proof.
-  intros Σ Re Rle Γ Δ h.
-  induction h. all: simpl ; auto.
-Qed.
+  Lemma eq_context_upto_sym Σ R pb :
+    RelationClasses.Symmetric (R Conv) ->
+    RelationClasses.Symmetric (R pb) ->
+    Symmetric (eq_context_upto Σ R pb).
+  Proof. tc. Qed.
 
-Lemma eq_context_upto_subst_context Σ Re Rle :
-  RelationClasses.subrelation Re Rle ->
-  forall u v n l l',
-    eq_context_upto Σ Re Rle u v ->
-    All2 (eq_term_upto_univ Σ Re Re) l l' ->
-    eq_context_upto Σ Re Rle (subst_context l n u) (subst_context l' n v).
-Proof.
-  intros re u v n l l'.
-  induction 1; intros Hl.
-  - rewrite !subst_context_nil. constructor.
-  - rewrite !subst_context_snoc; constructor; eauto.
-    depelim p; constructor; simpl; intuition auto;
-    rewrite -(length_of X);
-    apply eq_term_upto_univ_substs; auto. reflexivity.
-Qed.
+  Lemma eq_context_upto_cat Σ R pb Γ Δ Γ' Δ' :
+    eq_context_upto Σ R pb Γ Γ' ->
+    eq_context_upto Σ R pb Δ Δ' ->
+    eq_context_upto Σ R pb (Γ ,,, Δ) (Γ' ,,, Δ').
+  Proof. intros. eapply All2_app; eauto. Qed.
 
-#[global]
-Hint Resolve All2_fold_nil : pcuic.
+  Lemma eq_context_upto_rev Σ R pb Γ Δ :
+    eq_context_upto Σ R pb Γ Δ ->
+    eq_context_upto Σ R pb (rev Γ) (rev Δ).
+  Proof.
+    induction 1.
+    - constructor.
+    - rewrite 2!rev_cons. eapply eq_context_upto_cat ; eauto.
+  Qed.
 
-Lemma eq_context_upto_smash_context Σ ctx ctx' x y :
-  eq_context_upto Σ eq eq ctx ctx' -> eq_context_upto Σ eq eq x y -> 
-  eq_context_upto Σ eq eq (smash_context ctx x) (smash_context ctx' y).
-Proof.
-  induction x in ctx, ctx', y |- *; intros eqctx eqt; inv eqt; simpl; 
-    try split; auto; try constructor; auto. depelim X0 => /=.
-  - apply IHx; auto. apply eq_context_upto_cat; auto.
-    constructor; pcuic.
-  - apply IHx; auto. eapply eq_context_upto_subst_context; eauto.
-    typeclasses eauto.
-Qed.
+  Lemma eq_context_upto_rev'  Σ Γ Δ R pb :
+      eq_context_upto Σ R pb Γ Δ ->
+      eq_context_upto Σ R pb (List.rev Γ) (List.rev Δ).
+  Proof.
+    induction 1.
+    - constructor.
+    - simpl. eapply eq_context_upto_cat.
+      + repeat constructor; assumption.
+      + assumption.
+  Qed.
 
-Lemma eq_context_upto_nth_error Σ Re Rle ctx ctx' n :
-  eq_context_upto Σ Re Rle ctx ctx' -> 
-  rel_option (eq_decl_upto_gen Σ Re Rle) (nth_error ctx n) (nth_error ctx' n).
-Proof.
-  induction 1 in n |- *.
-  - rewrite nth_error_nil. constructor.
-  - destruct n; simpl; auto. 
-    constructor. depelim p; constructor; intuition auto;
-    now constructor.
-Qed.
+  Lemma eq_context_upto_length {Σ Re Rle Γ Δ} :
+      eq_context_upto Σ Re Rle Γ Δ ->
+      #|Γ| = #|Δ|.
+  Proof.
+    eapply All2_length.
+  Qed.
 
-Lemma eq_context_impl :
-  forall Σ Re Re' Rle Rle',
-    RelationClasses.subrelation Re Re' ->
-    RelationClasses.subrelation Rle Rle' ->
-    RelationClasses.subrelation Re' Rle' ->
-    subrelation (eq_context_upto Σ Re Rle) (eq_context_upto Σ Re' Rle').
-Proof.
-  intros Σ Re Re' Rle Rle' hR hR' hReRle' Γ Δ h.
-  induction h.
-  - constructor.
-  - constructor; auto. 
-    depelim p; constructor; auto.
-    all:eapply eq_term_upto_univ_impl. 5,10,15:tea. all:eauto.
-    all:now transitivity Re'.
-Qed.
+  Lemma eq_context_upto_subst_context Σ R pb u v n l l' :
+    RelationClasses.subrelation (R Conv) (R pb) ->
+      eq_context_upto Σ R pb u v ->
+      All2 (compare_term_upto_univ Σ R Conv) l l' ->
+      eq_context_upto Σ R pb (subst_context l n u) (subst_context l' n v).
+  Proof.
+    intros re.
+    induction 1; intros Hl.
+    - rewrite !subst_context_nil. constructor.
+    - rewrite !subst_context_snoc; constructor; eauto.
+      depelim r; constructor; simpl; intuition auto.
+      all: rewrite -(All2_length X) ;
+      apply compare_term_upto_univ_substs; auto.
+      reflexivity.
+  Qed.
 
-Lemma eq_term_upto_univ_it_mkLambda_or_LetIn Σ Re Rle :
-    RelationClasses.Reflexive Re ->
-    Proper (eq_context_upto Σ Re Re ==> eq_term_upto_univ Σ Re Rle ==> eq_term_upto_univ Σ Re Rle) it_mkLambda_or_LetIn.
-Proof.
-  intros he Γ Δ eq u v h.
-  induction eq in u, v, h, he |- *.
-  - assumption.
-  - simpl. cbn. apply IHeq => //.
-    destruct p; cbn; constructor ; tas; try reflexivity.
-Qed.
+  #[global]
+  Hint Resolve All2_fold_nil : pcuic.
 
-Lemma eq_term_upto_univ_it_mkLambda_or_LetIn_r Σ Re Rle Γ :
-  RelationClasses.Reflexive Re ->
-  respectful (eq_term_upto_univ Σ Re Rle) (eq_term_upto_univ Σ Re Rle)
-             (it_mkLambda_or_LetIn Γ) (it_mkLambda_or_LetIn Γ).
-Proof.
-  intros he u v h.
-  induction Γ as [| [na [b|] A] Γ ih ] in u, v, h |- *.
-  - assumption.
-  - simpl. cbn. apply ih. constructor ; try apply eq_term_upto_univ_refl.
-    all: auto.
-  - simpl. cbn. apply ih. constructor ; try apply eq_term_upto_univ_refl.
-    all: auto.
-Qed.
+  Lemma eq_context_upto_smash_context ctx ctx' x y :
+    ctx ≡Γ ctx' -> x ≡Γ y -> 
+    smash_context ctx x ≡Γ smash_context ctx' y.
+  Proof.
+    induction x in ctx, ctx', y |- *; intros eqctx eqt; inv eqt; simpl; 
+      try split; auto; try constructor; auto. depelim X => /=.
+    - apply IHx; auto. apply eq_context_upto_cat; auto.
+      constructor; pcuic.
+    - apply IHx; auto. eapply eq_context_upto_subst_context; eauto.
+      typeclasses eauto.
+  Qed.
 
-Lemma eq_term_it_mkLambda_or_LetIn {cf:checker_flags} Σ φ Γ :
-  respectful (eq_term Σ φ) (eq_term Σ φ)
-             (it_mkLambda_or_LetIn Γ) (it_mkLambda_or_LetIn Γ).
-Proof.
-  apply eq_term_upto_univ_it_mkLambda_or_LetIn_r; exact _.
-Qed.
+  (* Lemma eq_context_upto_nth_error Σ Re Rle ctx ctx' n :
+    eq_context_upto Σ Re Rle ctx ctx' -> 
+    rel_option (eq_decl_upto_gen Σ Re Rle) (nth_error ctx n) (nth_error ctx' n).
+  Proof.
+    induction 1 in n |- *.
+    - rewrite nth_error_nil. constructor.
+    - destruct n; simpl; auto. 
+      constructor. depelim p; constructor; intuition auto;
+      now constructor.
+  Qed.*)
 
-Lemma eq_term_upto_univ_it_mkProd_or_LetIn Σ Re Rle Γ :
-  RelationClasses.Reflexive Re ->
-  respectful (eq_term_upto_univ Σ Re Rle) (eq_term_upto_univ Σ Re Rle)
-             (it_mkProd_or_LetIn Γ) (it_mkProd_or_LetIn Γ).
-Proof.
-  intros he u v h.
-  induction Γ as [| [na [b|] A] Γ ih ] in u, v, h |- *.
-  - assumption.
-  - simpl. cbn. apply ih. constructor ; try apply eq_term_upto_univ_refl.
-    all: auto.
-  - simpl. cbn. apply ih. constructor ; try apply eq_term_upto_univ_refl.
-    all: auto.
-Qed.
+  Lemma eq_context_impl Σ R R' pb:
+      RelationClasses.subrelation (R Conv) (R' Conv) ->
+      RelationClasses.subrelation (R Conv) (R' pb) ->
+      RelationClasses.subrelation (R pb) (R' pb) ->
+      subrelation (eq_context_upto Σ R pb) (eq_context_upto Σ R' pb).
+  Proof.
+    intros hR hR' hR'' Γ Δ h.
+    induction h.
+    - constructor.
+    - constructor; auto. 
+      depelim r; constructor; auto.
+      all:eapply compare_term_upto_univ_impl ; eauto with arith.
+  Qed.
 
-Lemma eq_term_it_mkProd_or_LetIn {cf:checker_flags} Σ φ Γ:
-  respectful (eq_term Σ φ) (eq_term Σ φ)
-             (it_mkProd_or_LetIn Γ) (it_mkProd_or_LetIn Γ).
-Proof.
-  eapply eq_term_upto_univ_it_mkProd_or_LetIn ; exact _.
-Qed.
-
-Lemma eq_term_it_mkLambda_or_LetIn_inv {cf:checker_flags} Σ φ Γ u v :
-    eq_term Σ φ (it_mkLambda_or_LetIn Γ u) (it_mkLambda_or_LetIn Γ v) ->
-    eq_term Σ  φ u v.
-Proof.
-  revert u v. induction Γ as [| [na [b|] A] Γ ih ] ; intros u v h.
-  - assumption.
-  - simpl in h. cbn in h. apply ih in h. inversion h. subst.
-    assumption.
-  - simpl in h. cbn in h. apply ih in h. inversion h. subst.
-    assumption.
-Qed.
-
-Lemma eq_term_upto_univ_mkApps_inv Σ Re Rle u l u' l' :
-  isApp u = false ->
-  isApp u' = false ->
-  eq_term_upto_univ Σ Re Rle (mkApps u l) (mkApps u' l') ->
-  eq_term_upto_univ_napp Σ Re Rle #|l| u u' * All2 (eq_term_upto_univ Σ Re Re) l l'.
-Proof.
-  intros hu hu' h.
-  apply eq_term_upto_univ_mkApps_l_inv in h as hh.
-  destruct hh as [v [args [[h1 h2] h3]]].
-  apply eq_term_upto_univ_isApp in h1 as hh1. rewrite hu in hh1.
-  apply mkApps_notApp_inj in h3 ; auto.
-  destruct h3 as [? ?]. subst. split ; auto.
-Qed.
-
-Lemma isLambda_eq_term_l Σ Re u v :
+Lemma isLambda_compare_term_l Σ R pb u v :
     isLambda u ->
-    eq_term_upto_univ Σ Re Re u v ->
+    compare_term_upto_univ Σ R pb u v ->
     isLambda v.
 Proof.
   intros h e.
@@ -1556,9 +1744,9 @@ Proof.
   depelim e. auto.
 Qed.
 
-Lemma isLambda_eq_term_r Σ Re u v :
+Lemma isLambda_compare_term_r Σ R pb u v :
     isLambda v ->
-    eq_term_upto_univ Σ Re Re u v ->
+    compare_term_upto_univ Σ R pb u v ->
     isLambda u.
 Proof.
   intros h e.
@@ -1566,9 +1754,9 @@ Proof.
   depelim e. auto.
 Qed.
 
-Lemma isConstruct_app_eq_term_l Σ Re u v :
+Lemma isConstruct_app_compare_term_l Σ R pb u v :
     isConstruct_app u ->
-    eq_term_upto_univ Σ Re Re u v ->
+    compare_term_upto_univ Σ R pb u v ->
     isConstruct_app v.
 Proof.
   intros h e.
@@ -1580,20 +1768,19 @@ Proof.
   destruct t1 ; try discriminate.
   apply decompose_app_inv in e1 as ?. subst.
   apply decompose_app_inv in e2 as ?. subst.
-  apply eq_term_upto_univ_mkApps_inv in e as hh.
+  apply compare_term_upto_univ_mkApps_inv in e as hh.
   - destruct hh as [h1 h2].
     dependent destruction h1. reflexivity.
   - reflexivity.
   - eapply decompose_app_notApp. eassumption.
 Qed.
 
-Lemma isConstruct_app_eq_term_r :
-  forall Σ Re u v,
-    isConstruct_app v ->
-    eq_term_upto_univ Σ Re Re u v ->
-    isConstruct_app u.
+Lemma isConstruct_app_compare_term_r Σ R pb u v :
+  isConstruct_app v ->
+  compare_term_upto_univ Σ R pb u v ->
+  isConstruct_app u.
 Proof.
-  intros Σ Re u v h e.
+  intros h e.
   case_eq (decompose_app u). intros t1 l1 e1.
   case_eq (decompose_app v). intros t2 l2 e2.
   unfold isConstruct_app in *.
@@ -1602,26 +1789,26 @@ Proof.
   destruct t2 ; try discriminate.
   apply decompose_app_inv in e1 as ?. subst.
   apply decompose_app_inv in e2 as ?. subst.
-  apply eq_term_upto_univ_mkApps_inv in e as hh.
+  apply compare_term_upto_univ_mkApps_inv in e as hh.
   - destruct hh as [h1 h2].
     dependent destruction h1. reflexivity.
   - eapply decompose_app_notApp. eassumption.
   - reflexivity.
 Qed.
 
-Lemma R_global_instance_flip Σ gr napp
-  (Re Rle Rle' : Universe.t -> Universe.t -> Prop) u v:
-  RelationClasses.Reflexive Re ->
-  RelationClasses.Reflexive Rle ->
-  RelationClasses.Symmetric Re ->
-  RelationClasses.Transitive Re ->
-  RelationClasses.Transitive Rle ->
-  RelationClasses.subrelation Re Rle ->
-  (forall x y, Rle x y -> Rle' y x) ->
-  R_global_instance Σ Re Rle gr napp u v ->
-  R_global_instance Σ Re Rle' gr napp v u.
+Lemma R_global_instance_flip Σ gr napp (R R' : conv_pb -> Universe.t -> Universe.t -> Prop) pb pb' u v:
+  RelationClasses.Reflexive (R Conv) ->
+  RelationClasses.Reflexive (R pb) ->
+  RelationClasses.Symmetric (R' Conv) ->
+  RelationClasses.Transitive (R Conv) ->
+  RelationClasses.Transitive (R pb) ->
+  RelationClasses.subrelation (R Conv) (R' Conv) ->
+  RelationClasses.subrelation (R Conv) (R pb') ->
+  (forall x y, (R pb x y) -> (R' pb' y x)) ->
+  R_global_instance Σ R pb gr napp u v ->
+  R_global_instance Σ R' pb' gr napp v u.
 Proof.
-  intros Rerefl Rlerefl Resym Retrans Rletrans incl incl'.
+  intros Rerefl Rlerefl Resym Retrans Rletrans inclc inclp incl'.
   rewrite /R_global_instance /R_opt_variance.
   destruct global_variance as [vs|] eqn:var.  
   - induction u in vs, v |- *; destruct v; simpl; auto;
@@ -1629,47 +1816,57 @@ Proof.
     intros [Ra Ru']. split.
     destruct v'; simpl; auto.
     apply IHu; auto.
-  - apply Forall2_symP; eauto.
+  - intros.
+    apply Forall2_symP; eauto.
+    eapply Forall2_impl ; eauto.
 Qed.
 
-Lemma eq_term_upto_univ_napp_flip Σ (Re Rle Rle' : Universe.t -> Universe.t -> Prop) napp u v :
-  RelationClasses.Reflexive Re ->
-  RelationClasses.Reflexive Rle ->
-  RelationClasses.Symmetric Re ->
-  RelationClasses.Transitive Re ->
-  RelationClasses.Transitive Rle ->
-  RelationClasses.subrelation Re Rle ->
-  (forall x y, Rle x y -> Rle' y x) ->
-  eq_term_upto_univ_napp Σ Re Rle napp u v ->
-  eq_term_upto_univ_napp Σ Re Rle' napp v u.
+Lemma compare_term_upto_univ_napp_flip Σ (R R' : conv_pb -> Universe.t -> Universe.t -> Prop) pb pb' napp u v :
+  RelationClasses.Reflexive (R Conv) ->
+  RelationClasses.Reflexive (R pb) ->
+  RelationClasses.Symmetric (R' Conv) ->
+  RelationClasses.Transitive (R Conv) ->
+  RelationClasses.Transitive (R pb) ->
+  RelationClasses.subrelation (R Conv) (R' Conv) ->
+  RelationClasses.subrelation (R Conv) (R pb') ->
+  (forall x y, (R pb x y) -> (R' pb' y x)) ->
+  compare_term_upto_univ_napp Σ R pb napp u v ->
+  compare_term_upto_univ_napp Σ R' pb' napp v u.
 Proof.
-  intros Rerefl Rlerefl Resym Retrans Rletrans incl incl' H.
-  assert (Resub : RelationClasses.subrelation Re Re).
-  { typeclasses eauto. }
-  revert Rerefl Rlerefl Resym Retrans Rletrans incl incl' Resub.
-  revert Re Rle u v H Rle'.
-  induction 1; intros; constructor; intuition auto.
-  all:try solve [now symmetry].
+  intros Rerefl Rlerefl Resym Retrans Rletrans incl incl' H e.
+  induction e in Rlerefl, Rletrans, incl', H |- *.
+  all: intros; constructor.
+  all: intuition auto.
+  all:try solve [symmetry ; eapply compare_term_upto_univ_impl ; [..|eassumption] ; auto ].
+  all:try solve [symmetry ; eapply R_universe_instance_impl ; [..|eassumption] ; auto].
+  all: try solve [now symmetry].
   all:eauto using R_global_instance_flip.
   - eapply All2_sym. solve_all.
-    * eapply eq_context_sym; try tc. tas. 
-    * now eapply eq_term_upto_univ_sym.
+    symmetry.
+    eapply compare_term_upto_univ_impl ; [..|eassumption] ; auto with arith.
+  - unfold eq_predicate in * ; intuition auto.
+    all: symmetry ; auto.
+    + solve_all.
+      now eapply compare_term_upto_univ_impl ; [..|eassumption].
+    + now eapply R_universe_instance_impl ; [..|eassumption].
+    + now eapply compare_term_upto_univ_impl ; [..|eassumption].
   - eapply All2_sym. solve_all.
-    now eapply eq_term_upto_univ_sym.
-    now eapply eq_term_upto_univ_sym.
-    now symmetry.
+    + now symmetry.
+    + symmetry. now eapply compare_term_upto_univ_impl ; [..|eassumption].
   - eapply All2_sym. solve_all.
-    now eapply eq_term_upto_univ_sym.
-    now eapply eq_term_upto_univ_sym.
-    now symmetry.
+    all: symmetry ; auto.
+    all: now eapply compare_term_upto_univ_impl ; [..|eassumption].
+  - eapply All2_sym. solve_all.
+      all: symmetry ; auto.
+      all: now eapply compare_term_upto_univ_impl ; [..|eassumption].
 Qed.
 
-Lemma eq_univ_make :
-  forall u u',
+Lemma eq_univ_make u u' : 
     Forall2 eq (map Universe.make u) (map Universe.make u') ->
     u = u'.
 Proof.
-  intros u u' H. eapply Forall2_map' in H.
+  intros H.
+  eapply Forall2_map' in H.
   eapply Forall2_eq. eapply Forall2_impl; tea.
   clear. intros [] [] H; now inversion H.
 Qed.
@@ -1678,11 +1875,11 @@ Qed.
 Notation eq_annots Γ Δ :=
   (Forall2 (fun na decl => eq_binder_annot na (decl_name decl)) Γ Δ).
 
-Lemma eq_context_gen_binder_annot Γ Δ : 
-  eq_context_gen eq eq Γ Δ -> eq_annots (forget_types Γ) Δ.
+Lemma eq_context_gen_binder_annot (pb : conv_pb) Γ Δ : 
+  eq_context_pb (fun _ => eq) pb Γ Δ -> eq_annots (forget_types Γ) Δ.
 Proof.
   induction 1; constructor; auto.
-  destruct p; auto.
+  destruct r; auto.
 Qed.
 
 Lemma eq_annots_fold (Γ : list aname) (f : nat -> term -> term) (Δ : context) : 
